This commit comes after adding the check in the `thunkLang` semantics that `Force` cannot return a thunk:   - Proofs regarding `thunkLang` were modified to work with the changes.   - A new delayed top-level semantics was added for `thunkLang` to allow     the `thunk_unthunk` proof to work, and an `undelay_next` proof was     added that converts between these semantics and the normal top-level     semantics.   - Wrapping of monads with `Ret`s was transferred from     `pure_to_thunk_1` to `thunk_unthunk`.   - In `pure_to_thunk_2`, the `thunk_unthunk` step now comes right after     `pure_to_thunk_1` and the `undelay` step sits between `thunk_unthunk`     and the rest of the steps.   - A new check that `Cons`' arguments are delayed was added in the     semantics. Proofs up to and including `pure_to_thunk2` complete without cheats. There are still cheats in `thunk_Let_Delay_VarScript` and `thunk_Delay_LamScript` whose proofs are trickier.

compiler/backend/languages/semantics/envLangScript.sml
@@ -267,7 +267,10 @@ Definition eval_to_def:
        Cons s =>
            do
              vs <- result_map (λx. eval_to k env x) xs;
-             return (Constructor s vs)
+             if EVERY is_anyThunk vs then
+               return (Constructor s vs)
+             else
+               fail Type_error
            od
        | If => fail Type_error
        | Seq => fail Type_error
@@ -396,7 +399,17 @@ Proof
         \\ rw [] \\ gs [])
       \\ fs [DECIDE “A ⇒ ¬MEM a b ⇔ MEM a b ⇒ ¬A”]
       \\ IF_CASES_TAC \\ gs []
-      \\ rw [MAP_MAP_o, combinTheory.o_DEF, MAP_EQ_f])
+      \\ rw [MAP_MAP_o, combinTheory.o_DEF, MAP_EQ_f]
+      \\ (
+        gvs [EVERY_EL, EL_MAP, EXISTS_MEM, MEM_MAP, MEM_EL]
+        \\ first_x_assum $ drule_then assume_tac \\ gvs []
+        \\ rpt (first_x_assum $ qspec_then ‘EL n xs’ assume_tac) \\ gvs []
+        \\ pop_assum $ drule_at_then Any assume_tac \\ gvs []
+        \\ rpt (
+          qpat_x_assum ‘_ ⇒ _’ mp_tac \\ impl_tac >- (qexists ‘n’ \\ simp [])
+          \\ strip_tac)
+        \\ Cases_on ‘eval_to k env (EL n xs)’
+        \\ Cases_on ‘eval_to j env (EL n xs)’ \\ gvs []))
     >- ((* IsEq *)
       gvs [LENGTH_EQ_NUM_compute]
       \\ rename1 ‘eval_to (k - 1) env x’
