compiler/backend/languages/semantics/thunk_semantics_delayedScript.sml
@@ -1,0 +1,861 @@
+open HolKernel Parse boolLib bossLib BasicProvers intLib;
+open stringTheory optionTheory sumTheory pairTheory listTheory rich_listTheory
+     alistTheory itreeTheory thunkLangTheory thunkLang_primitivesTheory
+     thunk_semanticsTheory;
+
+val _ = new_theory "thunk_semantics_delayed";
+
+val _ = set_grammar_ancestry ["thunkLang", "thunk_semantics"];
+
+Definition next_delayed_def:
+  next_delayed (k:num) sv stack (state:state) =
+    case sv of
+      INL Diverge => Div
+    | INL _ => Err
+    | INR v =>
+      case v of
+        Monadic mop vs => (
+          if mop = Ret ∧ LENGTH vs = 1 then
+            with_value (HD vs) (λv.
+              if ¬is_anyThunk v then Err else
+              case stack of
+                Done => Ret
+              | BC f fs =>
+                  if k = 0 then Div else
+                    apply_closure f v (λw. next_delayed (k - 1) w fs state)
+              | HC f fs =>
+                  if k = 0 then Div else next_delayed (k - 1) sv fs state)
+          else if mop = Raise ∧ LENGTH vs = 1  then
+            with_value (HD vs) (λv.
+              if ¬is_anyThunk v then Err else
+              case stack of
+                Done => Ret
+              | BC f fs =>
+                  if k = 0 then Div else next_delayed (k - 1) sv fs state
+              | HC f fs =>
+                  if k = 0 then Div else
+                  apply_closure f v (λw. next_delayed (k - 1) w fs state))
+          else if mop = Bind ∧ LENGTH vs = 2 then
+            (let m = EL 0 vs in
+             let f = EL 1 vs in
+               if k = 0 then Div else
+                 next_delayed (k - 1) (eval m) (BC f stack) state)
+          else if mop = Handle ∧ LENGTH vs = 2 then
+            (let m = EL 0 vs in
+             let f = EL 1 vs in
+               if k = 0 then Div else
+                 next_delayed (k - 1) (eval m) (HC f stack) state)
+          else if mop = Act ∧ LENGTH vs = 1 then
+            (with_atoms vs (λas.
+               case HD as of
+                 Msg channel content => Act (channel, content) stack state
+               | _ => Err))
+          else if mop = Alloc ∧ LENGTH vs = 2 then
+            (case result_map eval vs of
+               INR [vl; v] =>
+                (if ¬is_anyThunk v then Err else
+                 (case get_atoms [vl] of
+                    SOME [Int len] =>
+                      let n = if len < 0 then 0 else Num len in
+                      let new_state = state ++ [REPLICATE n v] in
+                      if k = 0 then Div else
+                      next_delayed (k-1)
+                        (INR $ Monadic Ret [Delay $ Lit (Loc (LENGTH state))])
+                        stack new_state
+                  | _ => Err))
+             | INL Diverge => Div
+             | _ => Err)
+          else if mop = Length ∧ LENGTH vs = 1 then
+            (with_atoms vs (λas.
+               case HD as of
+                 Loc n =>
+                   (if LENGTH state ≤ n then Err else
+                    if k = 0 then Div else
+                      next_delayed (k-1)
+                        (INR $ Monadic Ret [
+                            Delay $ Lit (Int (& (LENGTH (EL n state))))])
+                        stack state)
+               | _ => Err))
+          else if mop = Deref ∧ LENGTH vs = 2 then
+            (with_atoms vs (λas.
+               case (EL 0 as, EL 1 as) of
+                 (Loc n, Int i) =>
+                   (if LENGTH state ≤ n then Err else
+                    if k = 0 then Div else
+                    if 0 ≤ i ∧ i < & LENGTH (EL n state) then
+                      next_delayed (k - 1)
+                        (INR $ Monadic Ret [Value $ EL (Num i) (EL n state)])
+                        stack state
+                    else
+                      next_delayed (k - 1)
+                        (INR $ Monadic Raise [Delay $ Cons "Subscript" []])
+                        stack state)
+               | _ => Err))
+          else if mop = Update ∧ LENGTH vs = 3 then
+            (case result_map eval vs of
+               INR [vl; vi; v] =>
+                 (if ¬is_anyThunk v then Err else
+                    (case get_atoms [vl; vi] of
+                       SOME [Loc n; Int i] =>
+                         if LENGTH state ≤ n then Err else
+                         if k = 0 then Div else
+                         if 0 ≤ i ∧ i < & LENGTH (EL n state) then
+                           let new_state =
+                             LUPDATE (LUPDATE v (Num i) (EL n state)) n state
+                           in next_delayed (k - 1)
+                                (INR $ Monadic Ret [Delay $ Cons "" []])
+                                stack new_state
+                         else
+                           next_delayed (k - 1)
+                             (INR $ Monadic Raise [Delay $ Cons "Subscript" []])
+                             stack state
+                     | _ => Err))
+             | INL Diverge => Div
+             | _ => Err)
+          else Err)
+      | _ => Err
+End
+
+Definition next_action_delayed_def:
+  next_action_delayed sv stack state =
+    case some k. next_delayed k sv stack state ≠ Div of
+      NONE => Div
+    | SOME k => next_delayed k sv stack state
+End
+
+Definition interp'_delayed_def:
+  interp'_delayed =
+    itree_unfold_err
+      (λ(sv,stack,state).
+        case next_action_delayed sv stack state of
+          Ret => Ret' pure_semantics$Termination
+        | Err => Ret' pure_semantics$Error
+        | Div => Div'
+        | Act a new_stack new_state =>
+            Vis' a
+              (λy. (INR $ Monadic Ret [Delay $ Lit (Str y)],
+                    new_stack, new_state)))
+      ((λ_ ret. STRLEN ret ≤ max_FFI_return_size),
+       pure_semantics$FinalFFI,
+       λs. pure_semantics$FinalFFI s pure_semantics$FFI_failure)
+End
+
+Definition interp_delayed:
+  interp_delayed sv stack state = interp'_delayed (sv, stack, state)
+End
+
+Theorem interp_delayed_def:
+  interp_delayed sv stack state =
+    case next_action_delayed sv stack state of
+      Ret => Ret pure_semantics$Termination
+    | Div => Div
+    | Err => Ret pure_semantics$Error
+    | Act a new_stack new_state =>
+        Vis a (λs. case s of
+            INL x =>
+              Ret $ pure_semantics$FinalFFI a x
+          | INR y =>
+              if STRLEN y ≤ max_FFI_return_size then
+                interp_delayed (INR $ Monadic Ret [Delay $ Lit (Str y)])
+                               new_stack new_state
+              else Ret $ pure_semantics$FinalFFI a pure_semantics$FFI_failure)
+Proof
+  rw [Once interp_delayed, interp'_delayed_def]
+  \\ once_rewrite_tac [itree_unfold_err] \\ gvs []
+  \\ CASE_TAC \\ gvs [combinTheory.o_DEF, FUN_EQ_THM] \\ rw []
+  \\ CASE_TAC \\ gvs [] \\ CASE_TAC \\ gvs []
+  \\ rw [Once interp_delayed, interp'_delayed_def]
+QED
+
+Definition semantics_delayed_def:
+  semantics_delayed e stack state = interp_delayed (eval e) stack state
+End
+
+Definition itree_of_delayed_def:
+  itree_of_delayed e = semantics_delayed e Done []
+End
+
+Theorem next_delayed_less_eq:
+  ∀n e k st m.
+    next_delayed n e k st ≠ Div ∧
+    n ≤ m ⇒
+      next_delayed n e k st = next_delayed m e k st
+Proof
+  recInduct next_delayed_ind \\ rw []
+  \\ ntac 2 $ pop_assum mp_tac
+  \\ once_rewrite_tac [next_delayed_def]
+  \\ TOP_CASE_TAC \\ gvs [] \\ TOP_CASE_TAC \\ gvs []
+  \\ rename1 ‘s = Ret’
+  \\ Cases_on ‘s = Bind’ >- (gvs [] \\ rw [])
+  \\ Cases_on ‘s = Handle’ >- (gvs [] \\ rw [])
+  \\ Cases_on ‘s = Act’ >- (gvs [] \\ rw [])
+  \\ Cases_on ‘s = Raise’ \\ gvs []
+  >- (
+    IF_CASES_TAC \\ gvs [] \\ simp [with_value_def]
+    \\ ntac 3 (TOP_CASE_TAC \\ gvs [])
+    >- (IF_CASES_TAC \\ gvs [] \\ first_x_assum drule \\ rw [])
+    \\ simp [apply_closure_def, with_value_def] \\ rpt $ TOP_CASE_TAC \\ gvs []
+    \\ first_x_assum drule \\ rw [])
+  \\ Cases_on ‘s = Ret’ \\ gvs []
+  >- (
+    IF_CASES_TAC \\ gvs [] \\ simp [with_value_def]
+    \\ ntac 3 (reverse TOP_CASE_TAC \\ gvs [])
+    >- (IF_CASES_TAC \\ gvs [] \\ first_x_assum drule \\ rw [])
+    \\ simp [apply_closure_def, with_value_def] \\ rpt $ TOP_CASE_TAC \\ gvs []
+    \\ first_x_assum drule \\ rw [])
+  \\ Cases_on ‘s = Alloc’ \\ gvs []
+  >- (
+    IF_CASES_TAC \\ gvs [] \\ rw [with_atoms_def, with_value_def]
+    \\ rpt (TOP_CASE_TAC \\ gvs []) \\ first_x_assum drule \\ simp [])
+  \\ Cases_on ‘s = Length’ \\ gvs []
+  >- (
+    IF_CASES_TAC \\ gvs [] \\ rw [with_atoms_def]
+    \\ ntac 5 (TOP_CASE_TAC \\ gvs [])
+    \\ first_x_assum irule \\ simp [] \\ qexists_tac ‘[Loc n]’ \\ simp [])
+  \\ Cases_on ‘s = Deref’ \\ gvs []
+  >- (
+    IF_CASES_TAC \\ gvs [] \\ rw [with_atoms_def]
+    \\ ntac 7 (TOP_CASE_TAC \\ gvs [])
+    \\ first_x_assum irule \\ simp []
+    \\ qexists_tac ‘[Loc n; Int i]’ \\ simp [])
+  \\ Cases_on ‘s = Update’ \\ gvs []
+  >- (
+    IF_CASES_TAC \\ gvs [] \\ rw [with_atoms_def, with_value_def]
+    \\ rpt (TOP_CASE_TAC \\ gvs [])
+    \\ first_x_assum irule \\ simp []
+    \\ qexists_tac ‘[Loc n; Int i]’ \\ simp [])
+QED
+
+Theorem next_delayed_next_delayed:
+  next_delayed n e k st ≠ Div ∧ next_delayed m e k st ≠ Div ⇒
+  next_delayed n e k st = next_delayed m e k st
+Proof
+  metis_tac [arithmeticTheory.LESS_EQ_CASES, next_delayed_less_eq]
+QED
+
+Definition sim_ok_delayed_def:
+  sim_ok_delayed allow_error Rv Re ⇔
+    (∀x y.
+       Re x y ∧
+       (¬allow_error ⇒ eval x ≠ INL Type_error) ⇒
+         ($= +++ Rv) (eval x) (eval y)) ∧
+    (∀vs ws x y.
+       LIST_REL Rv (MAP SND vs) (MAP SND ws) ∧
+       MAP FST vs = MAP FST ws ∧
+       EVERY (λ(n,v). n ∈ freevars x ⇒ is_anyThunk v) vs ∧
+       Re x y ⇒
+         Re (subst vs x) (subst ws y))
+End
+
+Definition cont_rel_delayed_def[simp]:
+  cont_rel_delayed Re Done Done = T ∧
+  cont_rel_delayed Re (BC v c) (BC w d) = (Re v w ∧ cont_rel_delayed Re c d) ∧
+  cont_rel_delayed Re (HC v c) (HC w d) = (Re v w ∧ cont_rel_delayed Re c d) ∧
+  cont_rel_delayed Re _ _ = F
+End
+
+Definition state_rel_delayed_def:
+  state_rel_delayed Rv =
+    LIST_REL (LIST_REL (λv w. is_anyThunk v ∧ Rv v w))
+End
+
+Definition next_rel_delayed_def[simp]:
+  next_rel_delayed Rv Re (thunk_semantics$Act a c s)
+                         (thunk_semantics$Act b d t) =
+    (a = b ∧ cont_rel_delayed Re c d ∧ state_rel_delayed Rv s t) ∧
+  next_rel_delayed Rv Re Ret Ret = T ∧
+  next_rel_delayed Rv Re Div Div = T ∧
+  next_rel_delayed Rv Re Err Err = T ∧
+  next_rel_delayed Rv Re (_: (string # string) next_res) _ = F
+End
+
+Definition rel_ok_delayed_def:
+  rel_ok_delayed allow_error Rv Re ⇔
+    (∀v w. Rv v w ⇒ (is_anyThunk v ⇔ is_anyThunk w)) ∧
+    (∀v1 w1 v2 w2 f g.
+       Re v1 w1 ∧
+       Rv v2 w2 ∧
+       (¬allow_error ⇒
+          apply_closure v1 v2 f ≠ Err ∧
+          f (INL Type_error) = Err) ∧
+       is_anyThunk v2 ∧
+       (∀(x : err + v) y.
+              ($= +++ Rv) x y ∧
+              (¬allow_error ⇒ f x ≠ Err) ⇒
+                next_rel_delayed Rv Re (f x) (g y)
+                ) ⇒
+         next_rel_delayed Rv Re (apply_closure v1 v2 f)
+                                (apply_closure w1 w2 g)) ∧
+    (∀s x w.
+       Rv (Closure s x) w ⇒
+         (∃t y. w = Closure t y) ∨ (∃g m. w = Recclosure g m)) ∧
+    (∀f n w.
+       Rv (Recclosure f n) w ⇒
+         (∃g m. w = Recclosure g m) ∨ (∃t y. w = Closure t y)) ∧
+    (∀s w.
+       Rv (Thunk s) w ⇒ (∃t. w = Thunk t) ∨ (∃v. w = DoTick v)) ∧
+    (∀x w.
+       Rv (Atom x) w ⇒ w = Atom x) ∧
+    (∀v w.
+       Rv (DoTick v) w ⇒
+         ¬allow_error ∨
+         (∃u. w = DoTick u)) ∧
+    (∀s vs w.
+       Rv (Constructor s vs) w ⇒ ∃ws. w = Constructor s ws ∧
+                                      LIST_REL Rv vs ws) ∧
+    (∀s x y.
+       x = y ⇒ Rv (Monadic s [Delay $ Lit x])
+                  (Monadic s [Delay $ Lit y])) ∧
+    (∀s t.
+       Rv (Monadic s [Delay $ Cons t []])
+          (Monadic s [Delay $ Cons t []])) ∧
+    (∀s x y.
+       Rv x y ∧
+       is_anyThunk x ⇒
+         Rv (Monadic s [Value x])
+            (Monadic s [Value y])) ∧
+    (∀mop vs w.
+       Rv (Monadic mop vs) w ⇒
+         (∃ws. w = Monadic mop ws ∧
+               LIST_REL Re vs ws))
+End
+
+Theorem rel_ok_delayed_get_atoms:
+  ∀x y.
+    rel_ok_delayed ae Rv Re ∧
+    LIST_REL Rv x y ∧
+    (∀z. MEM z x ⇒ ∀w. z ≠ DoTick w) ⇒
+       get_atoms x = get_atoms y
+Proof
+  ho_match_mp_tac get_atoms_ind \\ rw [] \\ fs [rel_ok_delayed_def] \\ gvs []
+  >~ [ ‘get_atoms (DoTick _::_)’] >- (
+    gvs [LIST_REL_EL_EQN, MEM_EL, PULL_EXISTS, SF DNF_ss])
+  \\ qpat_x_assum ‘∀v w. Rv v w ⇒ (is_anyThunk v ⇔ is_anyThunk w)’ kall_tac
+  \\ rpt (first_x_assum (drule_then assume_tac)) \\ gvs [get_atoms_def]
+  \\ metis_tac []
+QED
+
+Theorem sim_ok_delayed_next_delayed:
+  ∀k v c s w d t.
+    rel_ok_delayed allow_error Rv Re ∧
+    sim_ok_delayed allow_error Rv Re ∧
+    ($= +++ Rv) v w ∧
+    cont_rel_delayed Re c d ∧
+    state_rel_delayed Rv s t ∧
+    (¬allow_error ⇒ next_delayed k v c s ≠ Err) ⇒
+      next_rel_delayed Rv Re (next_delayed k v c s) (next_delayed k w d t)
+Proof
+  ho_match_mp_tac next_delayed_ind \\ rw []
+  \\ qpat_x_assum ‘(_ +++ _) _ _’ mp_tac
+  \\ Cases_on ‘v’ \\ Cases_on ‘w’ \\ simp []
+  >- (
+    rw [next_delayed_def]
+    \\ CASE_TAC \\ simp [])
+  \\ rename1 ‘Rv v w’
+  \\ Cases_on ‘(∃s x. v = Closure s x) ∨
+               (∃f n. v = Recclosure f n) ∨
+               (∃x. v = Thunk x) ∨ (∃x. v = Atom x) ∨
+               (∃nm vs. v = Constructor nm vs)’
+  >- (
+    qpat_x_assum ‘rel_ok_delayed _ _ _’ mp_tac \\ rw [rel_ok_delayed_def]
+    \\ rpt (first_x_assum (drule_all_then assume_tac)) \\ rw [] \\ fs []
+    \\ simp [next_delayed_def])
+  \\ Cases_on ‘∃x. v = DoTick x’
+  >- (
+    qpat_x_assum ‘rel_ok_delayed _ _ _’ mp_tac \\ rw [rel_ok_delayed_def]
+    \\ gvs [Once next_delayed_def]
+    \\ rpt (first_x_assum (drule_all_then assume_tac)) \\ rw [] \\ fs []
+    \\ simp [Once next_delayed_def] \\ simp [Once next_delayed_def])
+  \\ rfs []
+  \\ ‘∃mop vs. v = Monadic mop vs’ by (
+    ntac 5 (pop_assum mp_tac) \\ Cases_on ‘v’ \\ simp [] \\ fs [])
+  \\ rw []
+  \\ ‘∃ws. w = Monadic mop ws ∧ LIST_REL Re vs ws’
+    by (qpat_x_assum ‘Rv _ _’ mp_tac
+        \\ qpat_x_assum ‘rel_ok_delayed _ _ _’ mp_tac
+        \\ rw [rel_ok_delayed_def]
+        \\ rpt (first_x_assum drule) \\ rw [])
+  \\ rw []
+  \\ drule_then assume_tac LIST_REL_LENGTH
+  \\ once_rewrite_tac [next_delayed_def] \\ simp []
+  \\ IF_CASES_TAC \\ simp []
+  >- ((* Ret *)
+    gvs [LENGTH_EQ_NUM_compute] \\ simp [with_value_def] \\ rename1 ‘Re v w’
+    \\ ‘($= +++ Rv) (eval v) (eval w)’ by (
+      fs [rel_ok_delayed_def] \\ first_x_assum drule \\ rw []
+      \\ gvs [sim_ok_delayed_def] \\ first_x_assum irule \\ simp []
+      \\ rw [] \\ CCONTR_TAC \\ fs [Once next_delayed_def, with_value_def])
+    \\ Cases_on ‘eval v’ \\ Cases_on ‘eval w’ \\ gvs [] >- (CASE_TAC \\ gvs [])
+    \\ ‘is_anyThunk y ⇔ is_anyThunk y'’ by gvs [rel_ok_delayed_def]
+    \\ IF_CASES_TAC \\ gvs []
+    \\ rw [] \\ reverse $ Cases_on ‘c’ \\ Cases_on ‘d’ \\ gvs [] \\ rw []
+    >- (
+      first_x_assum irule \\ rw [SF SFY_ss]
+      \\ gvs [Once next_delayed_def, with_value_def])
+    \\ fs [rel_ok_delayed_def]
+    \\ first_x_assum irule \\ rw [] \\ gvs []
+    >- (first_x_assum drule \\ rw [])
+    \\ fs [Once next_delayed_def, with_value_def])
+  \\ IF_CASES_TAC
+  >- ((* Raise *)
+    gvs [LENGTH_EQ_NUM_compute] \\ simp [with_value_def] \\ rename1 ‘Re v w’
+    \\ ‘($= +++ Rv) (eval v) (eval w)’ by (
+      fs [rel_ok_delayed_def] \\ first_x_assum drule \\ rw []
+      \\ gvs [sim_ok_delayed_def] \\ first_x_assum irule \\ simp []
+      \\ rw [] \\ CCONTR_TAC \\ fs [Once next_delayed_def, with_value_def])
+    \\ Cases_on ‘eval v’ \\ Cases_on ‘eval w’ \\ gvs [] >- (CASE_TAC \\ gvs [])
+    \\ ‘is_anyThunk y ⇔ is_anyThunk y'’ by gvs [rel_ok_delayed_def]
+    \\ rw [] \\ Cases_on ‘c’ \\ Cases_on ‘d’ \\ gvs [] \\ rw []
+    >- (first_x_assum irule \\ rw [SF SFY_ss]
+        \\ gvs [Once next_delayed_def, with_value_def])
+    \\ fs [rel_ok_delayed_def]
+    \\ first_x_assum irule \\ rw [] \\ gvs []
+    >- (first_x_assum drule \\ rw [])
+    \\ fs [Once next_delayed_def, with_value_def])
+  \\ IF_CASES_TAC
+  >- ((* Bind *)
+    rw []
+    \\ gvs [LIST_REL_EL_EQN, LENGTH_EQ_NUM_compute,
+            DECIDE “∀x. x < 2 ⇔ x = 0 ∨ x = 1”]
+    \\ fs [SF DNF_ss]
+    \\ first_x_assum irule \\ rw []
+    \\ fs [Once next_delayed_def]
+    \\ fs [sim_ok_delayed_def]
+    \\ first_x_assum irule \\ simp []
+    \\ fs [rel_ok_delayed_def] \\ first_x_assum drule \\ rw []
+    \\ fs [Once next_delayed_def]
+    \\ Cases_on ‘eval h’ \\ gvs [] \\ Cases_on ‘x’ \\ gvs [])
+  \\ IF_CASES_TAC
+  >- ((* Handle *)
+    rw []
+    \\ gvs [LIST_REL_EL_EQN, LENGTH_EQ_NUM_compute,
+            DECIDE “∀x. x < 2 ⇔ x = 0 ∨ x = 1”]
+    \\ fs [SF DNF_ss]
+    \\ first_x_assum irule \\ rw []
+    \\ fs [Once next_delayed_def]
+    \\ fs [sim_ok_delayed_def]
+    \\ first_x_assum irule \\ simp []
+    \\ fs [rel_ok_delayed_def] \\ first_x_assum drule \\ rw []
+    \\ fs [Once next_delayed_def]
+    \\ Cases_on ‘eval h’ \\ gvs [] \\ Cases_on ‘x’ \\ gvs [])
+  \\ IF_CASES_TAC
+  >- ((* Act *)
+    rw [] \\ gvs []
+    \\ gvs [LIST_REL_EL_EQN, LENGTH_EQ_NUM_compute, DECIDE “∀x. x < 1 ⇔ x = 0”]
+    \\ rename1 ‘Re v w’
+    \\ simp [with_atoms_def, result_map_def]
+    \\ ‘¬allow_error ⇒ eval v ≠ INL Type_error’
+      by (rpt strip_tac \\ gvs []
+          \\ gvs [Once next_delayed_def, with_atoms_def, result_map_def])
+    \\ ‘($= +++ Rv) (eval v) (eval w)’ by (
+      gvs [sim_ok_delayed_def] \\ first_x_assum irule
+      \\ fs [rel_ok_delayed_def] \\ first_x_assum drule \\ simp [])
+    \\ Cases_on ‘eval v’ \\ Cases_on ‘eval w’ \\ gvs []
+    >~ [‘eval _ = INL err’] >- (Cases_on ‘err’ \\ fs [])
+    \\ rename1 ‘eval v = INR a’  \\ rename1 ‘eval w = INR b’
+    \\ ‘¬allow_error ⇒ get_atoms [a] ≠ NONE’ by (
+      rpt strip_tac
+      \\ gvs [Once next_delayed_def, with_atoms_def, result_map_def])
+    \\ ‘∀x. a = Atom x ⇒ a = b’ by (rpt strip_tac \\ gvs [rel_ok_delayed_def])
+    \\ reverse (Cases_on ‘∃x. a = Atom x’) \\ gvs [get_atoms_def] >- (
+      ‘get_atoms [a] = NONE’ by (Cases_on ‘a’ \\ fs [get_atoms_def])
+      \\ simp []
+      \\ Cases_on ‘b’ \\ gvs [get_atoms_def]
+      \\ Cases_on ‘a’ \\ fs [get_atoms_def, rel_ok_delayed_def]
+      \\ rpt (first_x_assum (drule_then assume_tac)) \\ rw [])
+    \\ CASE_TAC \\ fs [])
+  \\ IF_CASES_TAC
+  >- ((* Alloc *)
+    rw [] \\ gvs []
+    \\ gvs [LIST_REL_EL_EQN, LENGTH_EQ_NUM_compute,
+            DECIDE “∀x. x < 2 ⇔ x = 0 ∨ x = 1”]
+    \\ gvs [SF DNF_ss]
+    \\ rename1 ‘Rv (_ _ [v1; v2]) (_ _ [w1; w2])’
+    \\ gvs [with_atoms_def, result_map_def]
+    \\ ‘¬allow_error ⇒ eval v1 ≠ INL Type_error ∧ eval v2 ≠ INL Type_error’
+      by (rpt strip_tac \\ gvs []
+          \\ gvs [Once next_delayed_def, with_atoms_def, result_map_def])
+    \\ ‘($= +++ Rv) (eval v1) (eval w1)’ by (
+      gvs [sim_ok_delayed_def] \\ first_x_assum irule
+      \\ fs [rel_ok_delayed_def] \\ first_x_assum drule \\ simp [])
+    \\ ‘($= +++ Rv) (eval v2) (eval w2)’ by (
+      gvs [sim_ok_delayed_def] \\ first_x_assum irule
+      \\ fs [rel_ok_delayed_def] \\ first_x_assum rev_drule \\ simp [])
+    \\ ‘∀err. eval v1 = INL err ⇔ eval w1 = INL err’ by (
+      Cases_on ‘eval v1’ \\ Cases_on ‘eval w1’ \\ gvs [])
+    \\ ‘∀err. eval v2 = INL err ⇔ eval w2 = INL err’ by (
+      Cases_on ‘eval v2’ \\ Cases_on ‘eval w2’ \\ gvs [])
+    \\ IF_CASES_TAC \\ gvs [] \\ IF_CASES_TAC \\ gvs []
+    \\ Cases_on ‘eval v1’ \\ gvs []
+    >~ [‘eval _ = INL err’] >- (Cases_on ‘err’ \\ gvs [SF DNF_ss, EQ_IMP_THM])
+    \\ Cases_on ‘eval v2’ \\ gvs []
+    >~ [‘eval _ = INL err’] >- (Cases_on ‘err’ \\ gvs [SF DNF_ss, EQ_IMP_THM])
+    \\ Cases_on ‘eval w1’ \\ gvs [] \\ Cases_on ‘eval w2’ \\ gvs []
+    \\ rename1 ‘eval v1 = INR a’  \\ rename1 ‘eval w1 = INR b’
+    \\ ‘is_anyThunk y' ⇔ is_anyThunk y'3'’ by gvs [rel_ok_delayed_def]
+    \\ ‘¬allow_error ⇒ get_atoms [a] ≠ NONE’ by (
+      rpt strip_tac
+      \\ gvs [Once next_delayed_def, with_atoms_def, result_map_def])
+    \\ ‘∀x. a = Atom x ⇒ a = b’ by (rpt strip_tac \\ gvs [rel_ok_delayed_def])
+    \\ reverse (Cases_on ‘∃x. a = Atom x’) \\ gvs [get_atoms_def]
+    >- (
+      ‘get_atoms [a] = NONE’ by (Cases_on ‘a’ \\ fs [get_atoms_def])
+      \\ simp []
+      \\ Cases_on ‘b’ \\ gvs [get_atoms_def]
+      \\ Cases_on ‘a’ \\ fs [get_atoms_def, rel_ok_delayed_def]
+      \\ rpt (first_x_assum (drule_then assume_tac)) \\ rw [])
+    \\ IF_CASES_TAC \\ gvs []
+    \\ BasicProvers.TOP_CASE_TAC \\ gvs []
+    \\ BasicProvers.TOP_CASE_TAC \\ gvs []
+    \\ first_x_assum irule
+    \\ gvs [state_rel_delayed_def, LIST_REL_REPLICATE_same, LIST_REL_EL_EQN,
+            rel_ok_delayed_def]
+    \\ rw [] \\ gvs []
+    \\ qpat_x_assum ‘next_delayed _ _ _ _ ≠ _’ mp_tac
+    \\ simp [Once next_delayed_def, with_atoms_def, result_map_def,
+             get_atoms_def, with_value_def])
+  \\ IF_CASES_TAC
+  >- ((* Length *)
+    rw [] \\ gvs []
+    \\ gvs [LIST_REL_EL_EQN, LENGTH_EQ_NUM_compute, DECIDE “∀x. x < 1 ⇔ x = 0”]
+    \\ rename1 ‘Re v w’
+    \\ simp [with_atoms_def, result_map_def]
+    \\ ‘¬allow_error ⇒ eval v ≠ INL Type_error’ by (
+      rpt strip_tac \\ gvs []
+      \\ gvs [Once next_delayed_def, with_atoms_def, result_map_def])
+    \\ ‘($= +++ Rv) (eval v) (eval w)’ by (
+      gvs [sim_ok_delayed_def] \\ first_x_assum irule
+      \\ fs [rel_ok_delayed_def] \\ first_x_assum drule \\ simp [])
+    \\ Cases_on ‘eval v’ \\ Cases_on ‘eval w’ \\ gvs []
+    >~ [‘eval _ = INL err’] >- (Cases_on ‘err’ \\ gvs [])
+    \\ rename1 ‘eval v = INR a’  \\ rename1 ‘eval w = INR b’
+    \\ ‘¬allow_error ⇒ get_atoms [a] ≠ NONE’ by (
+      rpt strip_tac
+      \\ gvs [Once next_delayed_def, with_atoms_def, result_map_def])
+    \\ ‘∀x. a = Atom x ⇒ a = b’ by (rpt strip_tac \\ gvs [rel_ok_delayed_def])
+    \\ reverse (Cases_on ‘∃x. a = Atom x’) \\ gvs [get_atoms_def]
+    >- (
+      ‘get_atoms [a] = NONE’ by (Cases_on ‘a’ \\ fs [get_atoms_def])
+      \\ simp []
+      \\ Cases_on ‘b’ \\ gvs [get_atoms_def]
+      \\ Cases_on ‘a’ \\ fs [get_atoms_def, rel_ok_delayed_def]
+      \\ rpt (first_x_assum (drule_then assume_tac)) \\ rw [])
+    \\ ‘LENGTH s = LENGTH t’ by gvs [state_rel_delayed_def, LIST_REL_EL_EQN]
+    \\ Cases_on ‘k = 0’ \\ fs [] \\ CASE_TAC \\ fs []
+    \\ IF_CASES_TAC \\ gvs []
+    \\ first_x_assum (resolve_then Any irule HD) \\ simp []
+    \\ gvs [state_rel_delayed_def, LIST_REL_REPLICATE_same,  LIST_REL_EL_EQN,
+            rel_ok_delayed_def]
+    \\ strip_tac
+    \\ gvs [Once next_delayed_def,
+            with_atoms_def, result_map_def, get_atoms_def])
+  \\ IF_CASES_TAC
+  >- ((* Deref *)
+    rw [] \\ gvs []
+    \\ gvs [LIST_REL_EL_EQN, LENGTH_EQ_NUM_compute,
+            DECIDE “∀x. x < 2 ⇔ x = 0 ∨ x = 1”]
+    \\ gvs [SF DNF_ss]
+    \\ rename1 ‘Rv (_ _ [v1; v2]) (_ _ [w1; w2])’
+    \\ simp [with_atoms_def, result_map_def]
+    \\ ‘¬allow_error ⇒ eval v1 ≠ INL Type_error’ by (
+      rpt strip_tac \\ gvs []
+      \\ gvs [Once next_delayed_def, with_atoms_def, result_map_def])
+    \\ ‘¬allow_error ⇒ eval v2 ≠ INL Type_error’ by (
+      rpt strip_tac \\ gvs []
+      \\ gvs [Once next_delayed_def, with_atoms_def, result_map_def])
+    \\ ‘($= +++ Rv) (eval v1) (eval w1)’ by (
+      gvs [sim_ok_delayed_def] \\ first_x_assum irule
+      \\ fs [rel_ok_delayed_def] \\ first_x_assum drule \\ simp [])
+    \\ ‘($= +++ Rv) (eval v2) (eval w2)’ by (
+      gvs [sim_ok_delayed_def] \\ first_x_assum irule
+      \\ fs [rel_ok_delayed_def] \\ first_x_assum drule \\ simp [])
+    \\ Cases_on ‘eval v1’ \\ Cases_on ‘eval w1’ \\ gvs []
+    >~ [‘eval _ = INL err’] >- (
+      Cases_on ‘err = Type_error’ \\ fs []
+      \\ Cases_on ‘eval v2’ \\ Cases_on ‘eval w2’ \\ gvs []
+      >~ [‘eval _ = INL err’] >- (Cases_on ‘err’ \\ fs [])
+      \\ Cases_on ‘err’ \\ fs [])
+    \\ Cases_on ‘eval v2’ \\ Cases_on ‘eval w2’ \\ gvs []
+    >~ [‘eval _ = INL err’] >- (Cases_on ‘err’ \\ fs [])
+    \\ rename1 ‘eval v1 = INR a1’  \\ rename1 ‘eval w1 = INR b1’
+    \\ rename1 ‘eval v2 = INR a2’  \\ rename1 ‘eval w2 = INR b2’
+    \\ ‘¬allow_error ⇒ get_atoms [a1; a2] ≠ NONE’ by (
+      rpt strip_tac
+      \\ gvs [Once next_delayed_def, with_atoms_def, result_map_def])
+    \\ ‘∀x. a1 = Atom x ⇒ a1 = b1’ by (
+      rpt strip_tac \\ gvs [rel_ok_delayed_def])
+    \\ ‘∀x. a2 = Atom x ⇒ a2 = b2’ by (
+      rpt strip_tac \\ gvs [rel_ok_delayed_def])
+    \\ reverse (Cases_on ‘∃x. a1 = Atom x’) \\ fs []
+    >- (
+      Cases_on ‘∃y. b1 = Atom y’ \\ fs []
+      >- (
+        rw [] \\ fs [rel_ok_delayed_def]
+        \\ qpat_x_assum ‘Rv a1 b1’ assume_tac
+        \\ Cases_on ‘a1’ \\ fs []
+        \\ rpt (first_x_assum (drule_then assume_tac)) \\ rw []
+        \\ fs [get_atoms_def])
+      \\ ‘get_atoms [a1; a2] = NONE’ by (Cases_on ‘a1’ \\ fs [get_atoms_def])
+      \\ ‘get_atoms [b1; b2] = NONE’ by (Cases_on ‘b1’ \\ fs [get_atoms_def])
+      \\ simp [])
+    \\ reverse (Cases_on ‘∃x. a2 = Atom x’) \\ fs []
+    >- (
+      Cases_on ‘∃y. b2 = Atom y’ \\ fs []
+      >- (
+        rw [] \\ fs [rel_ok_delayed_def]
+        \\ qpat_x_assum ‘Rv a2 b2’ assume_tac
+        \\ Cases_on ‘a2’ \\ fs []
+        \\ rpt (first_x_assum (drule_then assume_tac)) \\ rw []
+        \\ fs [get_atoms_def])
+      \\ rw []
+      \\ ‘get_atoms [a2] = NONE’ by (Cases_on ‘a2’ \\ fs [get_atoms_def])
+      \\ ‘get_atoms [b2] = NONE’ by (Cases_on ‘b2’ \\ fs [get_atoms_def])
+      \\ gvs [] \\ simp [get_atoms_def])
+    \\ rw [] \\ simp [get_atoms_def]
+    \\ BasicProvers.TOP_CASE_TAC \\ fs []
+    \\ BasicProvers.TOP_CASE_TAC \\ fs []
+    \\ ‘LENGTH s = LENGTH t’ by fs [state_rel_delayed_def, LIST_REL_EL_EQN]
+    \\ IF_CASES_TAC \\ fs []
+    \\ IF_CASES_TAC \\ fs []
+    \\ qpat_x_assum ‘¬_ ⇒ next_delayed _ _ _ _ ≠ _’ mp_tac
+    \\ simp [Once next_delayed_def, with_atoms_def, result_map_def,
+             get_atoms_def]
+    \\ strip_tac
+    \\ ‘LENGTH (EL n t) = LENGTH (EL n s)’
+      by gvs [state_rel_delayed_def, LIST_REL_EL_EQN]
+    \\ rpt (first_x_assum (resolve_then Any assume_tac HD) \\ fs [])
+    \\ IF_CASES_TAC \\ fs []
+    >- (
+      first_x_assum irule \\ gvs [SF SFY_ss]
+      \\ fs [rel_ok_delayed_def]
+      \\ first_x_assum irule
+      \\ qpat_x_assum ‘state_rel_delayed _ _ _’ mp_tac
+      \\ rw [state_rel_delayed_def]
+      \\ fs [Once LIST_REL_EL_EQN]
+      \\ first_x_assum (qspec_then ‘n’ assume_tac) \\ gvs [LIST_REL_EL_EQN]
+      \\ first_x_assum $ qspec_then ‘Num i’ assume_tac \\ gvs []
+      \\ imp_res_tac integerTheory.NUM_POSINT_EXISTS \\ gvs [])
+    \\ first_x_assum irule \\ gvs [SF SFY_ss]
+    \\ fs [rel_ok_delayed_def] \\ intLib.COOPER_TAC)
+  \\ IF_CASES_TAC
+  >- ((* Update *)
+    rw [] \\ gvs []
+    \\ gvs [LIST_REL_EL_EQN, LENGTH_EQ_NUM_compute,
+            DECIDE “∀x. x < 3 ⇔ x = 0 ∨ x = 1 ∨ x = 2”]
+    \\ gvs [SF DNF_ss]
+    \\ rename1 ‘Rv (_ _ [v1; v2; v3]) (_ _ [w1; w2; w3])’
+    \\ simp [with_atoms_def, result_map_def]
+    \\ ‘¬allow_error ⇒ eval v1 ≠ INL Type_error ∧
+          eval v2 ≠ INL Type_error ∧eval v3 ≠ INL Type_error’ by (
+      rpt strip_tac \\ gvs []
+      \\ gvs [Once next_delayed_def, with_atoms_def, result_map_def])
+    \\ ‘($= +++ Rv) (eval v1) (eval w1)’ by (
+      gvs [sim_ok_delayed_def] \\ first_x_assum irule
+      \\ fs [rel_ok_delayed_def] \\ first_x_assum drule \\ simp [])
+    \\ ‘($= +++ Rv) (eval v2) (eval w2)’ by (
+      gvs [sim_ok_delayed_def] \\ first_x_assum irule
+      \\ fs [rel_ok_delayed_def] \\ first_x_assum rev_drule \\ simp [])
+    \\ ‘($= +++ Rv) (eval v3) (eval w3)’ by (
+      gvs [sim_ok_delayed_def] \\ first_x_assum irule
+      \\ fs [rel_ok_delayed_def] \\ first_x_assum rev_drule \\ simp [])
+    \\ ‘∀err. eval v1 = INL err ⇔ eval w1 = INL err’ by (
+      Cases_on ‘eval v1’ \\ Cases_on ‘eval w1’ \\ gvs [])
+    \\ ‘∀err. eval v2 = INL err ⇔ eval w2 = INL err’ by (
+      Cases_on ‘eval v2’ \\ Cases_on ‘eval w2’ \\ gvs [])
+    \\ ‘∀err. eval v3 = INL err ⇔ eval w3 = INL err’ by (
+      Cases_on ‘eval v3’ \\ Cases_on ‘eval w3’ \\ gvs [])
+    \\ IF_CASES_TAC \\ gvs [] \\ IF_CASES_TAC \\ gvs []
+    \\ Cases_on ‘eval v1’ \\ gvs []
+    >~ [‘eval _ = INL err’] >- (Cases_on ‘err’ \\ gvs [EQ_IMP_THM, SF DNF_ss])
+    \\ Cases_on ‘eval v2’ \\ gvs []
+    >~ [‘eval _ = INL err’] >- (Cases_on ‘err’ \\ gvs [EQ_IMP_THM, SF DNF_ss])
+    \\ Cases_on ‘eval v3’ \\ gvs []
+    >~ [‘eval _ = INL err’] >- (Cases_on ‘err’ \\ gvs [EQ_IMP_THM, SF DNF_ss])
+    \\ Cases_on ‘eval w1’ \\ gvs [] \\ Cases_on ‘eval w2’ \\ gvs []
+    \\ Cases_on ‘eval w3’ \\ gvs []
+    \\ rename1 ‘eval v1 = INR a1’ \\ rename1 ‘eval w1 = INR b1’
+    \\ rename1 ‘eval v2 = INR a2’ \\ rename1 ‘eval w2 = INR b2’
+    \\ ‘is_anyThunk y'' ⇔ is_anyThunk y'5'’ by gvs [rel_ok_delayed_def]
+    \\ ‘¬allow_error ⇒ get_atoms [a1; a2] ≠ NONE’ by (
+      rpt strip_tac
+      \\ gvs [Once next_delayed_def, with_atoms_def, result_map_def])
+    \\ ‘∀x. a1 = Atom x ⇒ a1 = b1’ by (
+      rpt strip_tac \\ gvs [rel_ok_delayed_def])
+    \\ ‘∀x. a2 = Atom x ⇒ a2 = b2’ by (
+      rpt strip_tac \\ gvs [rel_ok_delayed_def])
+    \\ reverse (Cases_on ‘∃x. a1 = Atom x’) \\ fs []
+    >- (
+      Cases_on ‘∃y. b1 = Atom y’ \\ fs []
+      >- (
+        rw [] \\ fs [rel_ok_delayed_def]
+        \\ qpat_x_assum ‘Rv a1 b1’ assume_tac
+        \\ Cases_on ‘a1’ \\ fs []
+        \\ rpt (first_x_assum (drule_then assume_tac)) \\ rw []
+        \\ fs [get_atoms_def])
+      \\ ‘get_atoms [a1; a2] = NONE’ by (Cases_on ‘a1’ \\ fs [get_atoms_def])
+      \\ ‘get_atoms [b1; b2] = NONE’ by (Cases_on ‘b1’ \\ fs [get_atoms_def])
+      \\ simp [])
+    \\ reverse (Cases_on ‘∃x. a2 = Atom x’) \\ fs []
+    >- (
+      Cases_on ‘∃y. b2 = Atom y’ \\ fs []
+      >- (
+        rw [] \\ fs [rel_ok_delayed_def]
+        \\ qpat_x_assum ‘Rv a2 b2’ assume_tac
+        \\ Cases_on ‘a2’ \\ fs []
+        \\ rpt (first_x_assum (drule_then assume_tac)) \\ rw []
+        \\ fs [get_atoms_def])
+      \\ rw []
+      \\ ‘get_atoms [a2] = NONE’ by (Cases_on ‘a2’ \\ fs [get_atoms_def])
+      \\ ‘get_atoms [b2] = NONE’ by (Cases_on ‘b2’ \\ fs [get_atoms_def])
+      \\ gvs [] \\ simp [get_atoms_def])
+    \\ rw [] \\ simp [get_atoms_def]
+    \\ BasicProvers.TOP_CASE_TAC \\ fs []
+    \\ BasicProvers.TOP_CASE_TAC \\ fs []
+    \\ ‘LENGTH s = LENGTH t’ by fs [state_rel_delayed_def, LIST_REL_EL_EQN]
+    \\ IF_CASES_TAC \\ fs []
+    \\ IF_CASES_TAC \\ fs []
+    \\ qpat_x_assum ‘¬_ ⇒ next_delayed _ _ _ _ ≠ _’ mp_tac
+    \\ simp [Once next_delayed_def, with_value_def,
+             with_atoms_def, result_map_def, get_atoms_def]
+    \\ fs [result_map_def, get_atoms_def]
+    \\ strip_tac
+    \\ ‘LENGTH (EL n t) = LENGTH (EL n s)’
+      by gvs [state_rel_delayed_def, LIST_REL_EL_EQN]
+    \\ IF_CASES_TAC \\ fs []
+    >- (
+      first_x_assum irule \\ simp [result_map_def, get_atoms_def]
+      \\ gvs [state_rel_delayed_def, LIST_REL_EL_EQN, EL_LUPDATE]
+      \\ rw [] \\ gvs []
+      \\ rw [EL_LUPDATE] \\ fs [rel_ok_delayed_def])
+    >- (last_x_assum irule \\ fs [rel_ok_delayed_def])
+    >- (first_x_assum irule \\ fs [rel_ok_delayed_def]))
+  \\ fs []
+QED
+
+Theorem sim_ok_delayed_next_action_delayed:
+  rel_ok_delayed allow_error Rv Re ∧
+  sim_ok_delayed allow_error Rv Re ∧
+  ($= +++ Rv) v w ∧
+  cont_rel_delayed Re c d ∧
+  state_rel_delayed Rv s t ∧
+  (¬allow_error ⇒ next_action_delayed v c s ≠ Err) ⇒
+    next_rel_delayed Rv Re (next_action_delayed v c s)
+                           (next_action_delayed w d t)
+Proof
+  strip_tac
+  \\ rw [next_action_delayed_def]
+  \\ DEEP_INTRO_TAC some_intro \\ simp []
+  \\ DEEP_INTRO_TAC some_intro \\ simp []
+  \\ simp [PULL_FORALL]
+  \\ qx_gen_tac ‘i’
+  \\ qx_gen_tac ‘j’
+  \\ qx_gen_tac ‘k’
+  \\ ‘∀m. ¬allow_error ⇒ next_delayed m v c s ≠ Err’ by (
+    rpt strip_tac \\ gvs []
+    \\ gvs [next_action_delayed_def]
+    \\ qpat_x_assum ‘_ ≠ Err’ mp_tac
+    \\ DEEP_INTRO_TAC some_intro \\ simp []
+    \\ simp [PULL_EXISTS]
+    \\ qexists_tac ‘m’ \\ gvs []
+    \\ rw []
+    \\ drule_then (qspec_then ‘m’ assume_tac) next_delayed_next_delayed
+    \\ gvs [])
+  \\ rw []
+  >- (
+    first_x_assum (qspec_then ‘i’ assume_tac)
+    \\ drule_all_then assume_tac sim_ok_delayed_next_delayed \\ gvs []
+    \\ drule_then (qspec_then ‘i’ mp_tac) next_delayed_next_delayed
+    \\ impl_tac \\ rw []
+    \\ strip_tac
+    \\ Cases_on ‘next_delayed i w d t’ \\ gvs [])
+  >- (
+    last_x_assum (qspec_then ‘i’ assume_tac)
+    \\ drule_all_then assume_tac sim_ok_delayed_next_delayed \\ gvs [SF SFY_ss])
+  \\ last_x_assum (qspec_then ‘k’ assume_tac)
+  \\ drule_all_then assume_tac sim_ok_delayed_next_delayed \\ gvs [SF SFY_ss]
+QED
+
+Theorem sim_ok_delayed_interp_delayed:
+  rel_ok_delayed allow_error Rv Re ∧
+  sim_ok_delayed allow_error Rv Re ∧
+  ($= +++ Rv) v w ∧
+  cont_rel_delayed Re c d ∧
+  state_rel_delayed Rv s t ∧
+  (¬allow_error ⇒ pure_semantics$safe_itree (interp_delayed v c s)) ⇒
+    interp_delayed v c s = interp_delayed w d t
+Proof
+  strip_tac
+  \\ rw [Once itreeTheory.itree_bisimulation]
+  \\ qexists
+    ‘λt1 t2.
+      (¬allow_error ⇒ pure_semantics$safe_itree t1) ∧
+      (t1 = t2 ∨
+       ∃v c s w d t.
+         interp_delayed v c s = t1 ∧
+         interp_delayed w d t = t2 ∧
+         ($= +++ Rv) v w ∧
+         cont_rel_delayed Re c d ∧
+         state_rel_delayed Rv s t)’
+  \\ rw []
+  >~ [‘Vis a f’] >- (
+    rgs [Once pure_semanticsTheory.safe_itree_cases])
+  >~ [‘interp_delayed v c s = interp_delayed w d t’] >- (
+    disj2_tac \\ rpt $ irule_at Any EQ_REFL \\ simp [])
+  \\ ‘¬allow_error ⇒ next_action_delayed v' c' s' ≠ Err’ by (
+    rpt strip_tac \\ gvs []
+    \\ rgs [Once interp_delayed_def,
+            Once pure_semanticsTheory.safe_itree_cases])
+  \\ drule_all sim_ok_delayed_next_action_delayed \\ strip_tac
+  >- (
+    qpat_x_assum ‘_ = Ret _’ mp_tac
+    \\ once_rewrite_tac [interp_delayed_def]
+    \\ Cases_on ‘next_action_delayed v' c' s'’
+    \\ Cases_on ‘next_action_delayed w' d' t''’ \\ gvs [])
+  >- (
+    qpat_x_assum ‘_ = Div’ mp_tac
+    \\ once_rewrite_tac[interp_delayed_def]
+    \\ Cases_on ‘next_action_delayed v' c' s'’
+    \\ Cases_on ‘next_action_delayed w' d' t''’
+    \\ gvs [])
+  >- (
+    qpat_x_assum ‘_ = Vis _ _ ’ mp_tac
+    \\ rw [Once interp_delayed_def]
+    \\ rw [Once interp_delayed_def]
+    \\ Cases_on ‘next_action_delayed v' c' s'’
+    \\ Cases_on ‘next_action_delayed w' d' t''’ \\ gvs []
+    \\ rw [] \\ rgs [Once pure_semanticsTheory.safe_itree_cases]
+    \\ CASE_TAC \\ gvs [] \\ CASE_TAC \\ gvs []
+    \\ disj2_tac
+    \\ rpt (irule_at Any EQ_REFL) \\ simp []
+    \\ gvs [rel_ok_delayed_def])
+QED
+
+Theorem semantics_delayed_fail:
+  pure_semantics$safe_itree (semantics_delayed x c s) ⇒
+    eval x ≠ INL Type_error
+Proof
+  simp [semantics_delayed_def, Once interp_delayed_def, next_action_delayed_def]
+  \\ DEEP_INTRO_TAC some_intro \\ simp []
+  \\ rw [] \\ strip_tac \\ gvs []
+  \\ rgs [Once next_delayed_def]
+  \\ rgs [Once pure_semanticsTheory.safe_itree_cases]
+QED
+
+Theorem sim_ok_delayed_semantics_delayed:
+  rel_ok_delayed allow_error Rv Re ∧
+  sim_ok_delayed allow_error Rv Re ∧
+  Re x y ∧
+  (¬allow_error ⇒ pure_semantics$safe_itree (semantics_delayed x Done [])) ⇒
+    semantics_delayed x Done [] = semantics_delayed y Done []
+Proof
+  strip_tac
+  \\ rw [semantics_delayed_def]
+  \\ irule sim_ok_delayed_interp_delayed
+  \\ qpat_assum ‘sim_ok_delayed _ _ _’ (irule_at Any)
+  \\ gvs [cont_rel_delayed_def, state_rel_delayed_def, sim_ok_delayed_def]
+  \\ first_assum (irule_at Any) \\ gvs []
+  \\ rw [] \\ gvs [semantics_delayed_fail, SF SFY_ss]
+  \\ gvs [semantics_delayed_def]
+QED
+
+val _ = export_theory();
