compiler/backend/passes/proofs/pure_to_thunk_2ProofScript.sml
@@ -5,10 +5,12 @@
 open HolKernel Parse boolLib bossLib term_tactic monadsyntax dep_rewrite;
 open stringTheory optionTheory sumTheory pairTheory listTheory alistTheory
      finite_mapTheory pred_setTheory rich_listTheory arithmeticTheory combinTheory
-     pure_semanticsTheory thunkLangTheory thunk_semanticsTheory pure_evalTheory
+     pure_semanticsTheory pure_evalTheory
+     thunkLangTheory thunk_semanticsTheory thunk_semantics_delayedTheory
      thunkLang_primitivesTheory pure_exp_lemmasTheory pure_miscTheory
      pure_to_thunk_1ProofTheory pure_cexpTheory pureLangTheory
      thunk_unthunkProofTheory
+     thunk_undelay_nextProofTheory
      thunk_case_liftProofTheory
      thunk_case_projProofTheory thunk_exp_ofTheory
      thunk_let_forceProofTheory
@@ -121,32 +123,42 @@ Inductive exp_rel:
 End
 
 Overload to_thunk = “pure_to_thunk_1Proof$compile_rel”
+Overload delay_force = “thunk_unthunkProof$delay_force”
+Overload undelay = “thunk_undelay_nextProof$exp_rel”
 Overload lift_rel = “thunk_case_liftProof$compile_rel”
 Overload force_rel = “thunk_let_forceProof$exp_rel”
 Overload proj_rel = “thunk_case_projProof$compile_rel”
-Overload delay_force = “thunk_unthunkProof$delay_force”
 
 Overload VV[local] = “thunk_let_forceProof$Var”
 
 val to_thunk_freevars = pure_to_thunk_1ProofTheory.compile_rel_freevars;
 
+Theorem to_thunk_cases[local] = Once pure_to_thunk_1ProofTheory.compile_rel_cases;
+Theorem delay_force_cases[local] = Once thunk_unthunkProofTheory.delay_force_cases;
+Theorem undelay_cases[local] = Once thunk_undelay_nextProofTheory.exp_rel_cases;
+Theorem lift_cases[local] = Once thunk_case_liftProofTheory.compile_rel_cases;
+Theorem force_cases[local] = Once thunk_let_forceProofTheory.exp_rel_cases;
+Theorem proj_cases[local] = Once thunk_case_projProofTheory.compile_rel_cases;
+
 Theorem lets_for_lemma[local]:
   ∀vs k.
     to_thunk (exp_of' h2) y1 ∧
-    lift_rel y1 y2 ∧
-    force_rel NONE y2 y3 ∧
-    proj_rel y3 y4 ∧
-    delay_force y4 (exp_of yy2) ∧
+    delay_force y1 y2 ∧
+    undelay y2 y3 ∧
+    lift_rel y3 y4 ∧
+    force_rel NONE y4 y5 ∧
+    proj_rel y5 (exp_of yy2) ∧
     ~MEM fresh vs ∧ ~MEM h vs ∧ fresh ≠ h ∧ cn ∉ monad_cns ∧
     fresh ∉ freevars (exp_of' h2) ⇒
-    ∃x1 x2 x3 x4.
+    ∃x1 x2 x3 x4 x5.
       to_thunk
         (lets_for' (k + LENGTH vs) cn h
           (MAPi (λx v. (x+k,v)) vs) (exp_of' h2)) x1 ∧
-      lift_rel x1 x2 ∧ fresh ∉ freevars x1 ∧
-      force_rel (SOME (VV h,fresh)) x2 x3 ∧
-      proj_rel x3 x4 ∧
-      delay_force x4
+      delay_force x1 x2 ∧
+      undelay x2 x3 ∧
+      lift_rel x3 x4 ∧ fresh ∉ freevars x3 ∧
+      force_rel (SOME (VV h,fresh)) x4 x5 ∧
+      proj_rel x5
         (lets_for (k + LENGTH vs) cn fresh
           (MAPi (λx v. (x+k,v)) vs) (exp_of yy2))
 Proof
@@ -154,53 +166,40 @@ Proof
   \\ fs [lets_for_def,lets_for'_def]
   >-
    (rw [] \\ imp_res_tac to_thunk_freevars
-    \\ rpt $ first_x_assum $ irule_at Any \\ fs []
-    \\ irule thunk_let_forceProofTheory.exp_rel_NONE_IMP_SOME \\ fs [])
+    \\ rpt $ first_assum $ irule_at Any \\ fs []
+    \\ irule_at Any thunk_let_forceProofTheory.exp_rel_NONE_IMP_SOME \\ fs []
+    \\ imp_res_tac thunk_unthunkProofTheory.delay_force_freevars \\ fs []
+    \\ imp_res_tac thunk_undelay_nextProofTheory.exp_rel_freevars \\ fs [])
   \\ rw [] \\ gvs []
   \\ irule_at Any pure_to_thunk_1ProofTheory.compile_rel_Seq \\ fs []
-  \\ simp [Once pure_to_thunk_1ProofTheory.compile_rel_cases, PULL_EXISTS]
-  \\ simp [Once pure_to_thunk_1ProofTheory.compile_rel_cases, PULL_EXISTS]
-  \\ simp [Once pure_to_thunk_1ProofTheory.compile_rel_cases, PULL_EXISTS]
-  \\ simp [Once pure_to_thunk_1ProofTheory.compile_rel_cases, PULL_EXISTS]
-  \\ simp[pure_configTheory.monad_cns_def,
-         mop_rel_cases, mop_ret_rel_cases, mop_delay_rel_cases]
-  \\ simp [Once pure_to_thunk_1ProofTheory.compile_rel_cases, PULL_EXISTS]
+  \\ ntac 4 (simp [to_thunk_cases, PULL_EXISTS])
+  \\ simp[pure_configTheory.monad_cns_def, mop_rel_cases, mop_ret_rel_cases,
+          mop_delay_rel_cases]
+  \\ simp [to_thunk_cases, PULL_EXISTS]
   \\ irule_at Any pure_to_thunk_1ProofTheory.compile_rel_Let
   \\ irule_at Any pure_to_thunk_1ProofTheory.compile_rel_Proj \\ fs [PULL_EXISTS]
-  \\ irule_at Any pure_to_thunk_1ProofTheory.compile_rel_Var
+  \\ simp [to_thunk_cases, PULL_EXISTS]
   \\ irule_at Any thunk_case_projProofTheory.compile_rel_Proj \\ fs []
   \\ fs [o_DEF,freevars_def]
   \\ last_x_assum $ qspec_then ‘SUC k’ mp_tac
   \\ fs [ADD_CLAUSES] \\ rw []
-  \\ rpt $ first_x_assum $ irule_at Any
-  \\ irule_at Any thunk_case_liftProofTheory.compile_rel_Let
+  \\ ntac 2 (goal_assum drule)
+  \\ ntac 7 (simp [delay_force_cases, PULL_EXISTS])
+  \\ irule_at Any thunk_unthunkProofTheory.delay_force_Let
+  \\ ntac 5 (simp [delay_force_cases, PULL_EXISTS])
+  \\ ntac 5 (simp [undelay_cases, PULL_EXISTS])
+  \\ irule_at Any thunk_undelay_nextProofTheory.exp_rel_Prim \\ fs []
+  \\ ntac 7 (simp [undelay_cases, PULL_EXISTS])
+  \\ simp [lift_cases, PULL_EXISTS]
   \\ irule_at Any thunk_case_liftProofTheory.compile_rel_If \\ fs []
-  \\ irule_at Any thunk_case_liftProofTheory.compile_rel_Prim \\ fs [PULL_EXISTS]
-  \\ irule_at Any thunk_case_liftProofTheory.compile_rel_Prim \\ fs [PULL_EXISTS]
-  \\ irule_at Any thunk_case_liftProofTheory.compile_rel_Prim \\ fs [PULL_EXISTS]
-  \\ irule_at Any thunk_case_liftProofTheory.compile_rel_Force
-  \\ irule_at Any thunk_case_liftProofTheory.compile_rel_Var
-  \\ irule_at Any thunk_case_liftProofTheory.compile_rel_Let
-  \\ irule_at Any thunk_case_liftProofTheory.compile_rel_Delay
-  \\ irule_at Any thunk_case_liftProofTheory.compile_rel_Force
-  \\ irule_at Any thunk_case_liftProofTheory.compile_rel_Prim \\ fs [PULL_EXISTS]
-  \\ irule_at Any thunk_case_liftProofTheory.compile_rel_Force
-  \\ irule_at Any thunk_case_liftProofTheory.compile_rel_Var
-  \\ irule_at Any thunk_unthunkProofTheory.delay_force_Let
-  \\ irule_at Any thunk_unthunkProofTheory.delay_force_If \\ fs []
-  \\ irule_at Any thunk_unthunkProofTheory.delay_force_Prim \\ fs []
-  \\ irule_at Any thunk_unthunkProofTheory.delay_force_Prim \\ fs []
-  \\ irule_at Any thunk_unthunkProofTheory.delay_force_Var \\ fs []
-  \\ irule_at Any thunk_unthunkProofTheory.delay_force_Prim \\ fs []
-  \\ irule_at Any thunk_unthunkProofTheory.delay_force_Let
-  \\ irule_at Any thunk_unthunkProofTheory.delay_force_Prim \\ fs []
-  \\ irule_at Any thunk_unthunkProofTheory.delay_force_Var \\ fs []
-  \\ rpt $ first_x_assum $ irule_at Any
-  \\ irule_at Any thunk_let_forceProofTheory.exp_rel_Let
+  \\ ntac 11 (simp [lift_cases, PULL_EXISTS])
+  \\ fs [freevars_def]
+  \\ simp [force_cases, PULL_EXISTS]
   \\ fs [name_clash_def]
-  \\ irule_at Any thunk_let_forceProofTheory.exp_rel_Let
+  \\ ntac 6 (simp [force_cases, PULL_EXISTS])
   \\ fs [name_clash_def]
-  \\ rpt $ simp [Once thunk_let_forceProofTheory.exp_rel_cases]
+  \\ ntac 4 (simp [force_cases, PULL_EXISTS])
+  \\ rpt $ goal_assum drule
 QED
 
 Triviality MEM_EQ_MEM_MAP_explode:
@@ -224,6 +223,20 @@ Proof
   \\ simp[pure_configTheory.monad_cns_def]
 QED
 
+Theorem delay_force_Disj:
+  ∀xs v. delay_force (Disj' (Force (Var v)) xs) (Disj' (Force (Var v)) xs)
+Proof
+  Induct \\ fs [pureLangTheory.Disj_def, FORALL_PROD, Disj'_def] \\ rw []
+  \\ rpt (simp [Once thunk_unthunkProofTheory.delay_force_cases])
+QED
+
+Theorem undelay_Disj:
+  ∀xs v. undelay (Disj' (Force (Var v)) xs) (Disj' (Force (Var v)) xs)
+Proof
+  Induct \\ fs [pureLangTheory.Disj_def, FORALL_PROD, Disj'_def] \\ rw []
+  \\ rpt (simp [Once thunk_undelay_nextProofTheory.exp_rel_cases])
+QED
+
 Theorem lift_rel_Disj:
   ∀xs v. lift_rel (Disj' (Force (Var v)) xs) (Disj' (Force (Var v)) xs)
 Proof
@@ -243,18 +256,8 @@ Theorem proj_rel_Disj:
 Proof
   Induct \\ fs [Disj_def,FORALL_PROD] \\ rw []
   \\ rpt (irule_at Any thunk_case_projProofTheory.compile_rel_If \\ fs [])
-  \\ rpt (irule_at Any thunk_case_projProofTheory.compile_rel_Cons \\ fs [])
   \\ rpt (irule_at Any thunk_case_projProofTheory.compile_rel_Prim \\ fs [])
   \\ rpt (irule_at Any thunk_case_projProofTheory.compile_rel_Var \\ fs [])
-QED
-
-Theorem delay_force_Disj:
-  ∀xs v. delay_force (Disj v xs) (Disj v xs)
-Proof
-  Induct \\ fs [Disj_def,FORALL_PROD] \\ rw []
-  \\ rpt (irule_at Any thunk_unthunkProofTheory.delay_force_If \\ fs [])
-  \\ rpt (irule_at Any thunk_unthunkProofTheory.delay_force_Prim \\ fs [])
-  \\ rpt (irule_at Any thunk_unthunkProofTheory.delay_force_Var \\ fs [])
 QED
 
 Triviality freevars_Disj':
@@ -264,68 +267,57 @@ Proof
   \\ fs [freevars_def]
 QED
 
-Theorem to_thunk_cases[local] = Once pure_to_thunk_1ProofTheory.compile_rel_cases;
-Theorem lift_cases[local] = Once thunk_case_liftProofTheory.compile_rel_cases;
-Theorem force_cases[local] = Once thunk_let_forceProofTheory.exp_rel_cases;
-Theorem proj_cases[local] = Once thunk_case_projProofTheory.compile_rel_cases;
-Theorem delay_force_cases[local] = Once thunk_unthunkProofTheory.delay_force_cases;
-
 Theorem exp_rel_imp_combined:
   ∀x y.
     exp_rel x y ∧ cexp_wf x ⇒
-    ∃y1 y2 y3 y4.
+    ∃y1 y2 y3 y4 y5.
       to_thunk (exp_of' x) y1 ∧
-      lift_rel y1 y2 ∧
-      force_rel NONE y2 y3 ∧
-      proj_rel y3 y4 ∧
-      delay_force y4 (exp_of y)
+      delay_force y1 y2 ∧
+      undelay y2 y3 ∧
+      lift_rel y3 y4 ∧
+      force_rel NONE y4 y5 ∧
+      proj_rel y5 (exp_of y)
 Proof
   Induct_on ‘exp_rel’
-  \\ rw [exp_of'_def,pure_cexpTheory.cexp_wf_def] \\ fs [pure_cexpTheory.op_of_def]
-  >~ [‘Var n’] >-
-   (simp [Once pure_to_thunk_1ProofTheory.compile_rel_cases]
-    \\ irule_at Any thunk_unthunkProofTheory.delay_force_Force
-    \\ irule_at Any thunk_unthunkProofTheory.delay_force_Var
-    \\ irule_at Any thunk_case_liftProofTheory.compile_rel_Force
-    \\ irule_at Any thunk_case_liftProofTheory.compile_rel_Var
-    \\ irule_at Any thunk_let_forceProofTheory.exp_rel_Force
-    \\ irule_at Any thunk_let_forceProofTheory.exp_rel_Var
+  \\ rw [exp_of'_def,pure_cexpTheory.cexp_wf_def]
+  \\ fs [pure_cexpTheory.op_of_def]
+  >~ [‘Var n’] >- (
+    ntac 2 (simp [to_thunk_cases, delay_force_cases, undelay_cases, lift_cases,
+                  force_cases, proj_cases, PULL_EXISTS]))
+  >~ [‘rows_of'’] >- (
+    ntac 2 (irule_at Any thunk_case_projProofTheory.compile_rel_Let_SOME)
     \\ irule_at Any thunk_case_projProofTheory.compile_rel_Force
-    \\ irule_at Any thunk_case_projProofTheory.compile_rel_Var)
-  >~ [‘rows_of'’] >-
-   (irule_at Any thunk_case_projProofTheory.compile_rel_Let_SOME
-    \\ irule_at Any thunk_let_forceProofTheory.exp_rel_Let
+    \\ irule_at Any thunk_case_projProofTheory.compile_rel_Var
+    \\ irule_at Any pure_to_thunk_1ProofTheory.compile_rel_Let
+    \\ irule_at Any thunk_unthunkProofTheory.delay_force_Let
+    \\ irule_at Any thunk_undelay_nextProofTheory.exp_rel_Let
     \\ irule_at Any thunk_case_liftProofTheory.compile_rel_Let
-    \\ fs [name_clash_def]
-    \\ irule_at Any thunk_unthunkProofTheory.delay_force_Let
-    \\ simp [Once pure_to_thunk_1ProofTheory.compile_rel_cases,PULL_EXISTS]
-    \\ irule_at Any thunk_unthunkProofTheory.delay_force_Let
-    \\ irule_at Any thunk_unthunkProofTheory.delay_force_Force
-    \\ irule_at Any thunk_unthunkProofTheory.delay_force_Var
-    \\ irule_at Any thunk_case_liftProofTheory.compile_rel_Delay
-    \\ irule_at Any thunk_let_forceProofTheory.exp_rel_Delay
-    \\ irule_at Any thunk_case_projProofTheory.compile_rel_Delay
-    \\ gvs [PULL_EXISTS]
-    \\ ‘∃q1 q2 q3 q4.
+    \\ irule_at Any thunk_let_forceProofTheory.exp_rel_Let
+    \\ gvs [name_clash_def, PULL_EXISTS]
+    \\ `∃q1 q2 q3 q4 q5.
           to_thunk (exp_of' x) q1 ∧
-          lift_rel q1 q2 ∧
-          force_rel NONE q2 q3 ∧
-          proj_rel q3 q4 ∧
-          delay_force (Delay q4) (exp_of a_exp)’ by
-      (qpat_x_assum ‘(∀c z. x = Var c z ⇒ a_exp ≠ Var z) ⇒ _’ mp_tac
+          delay_force (Delay q1) q2 ∧
+          undelay q2 q3 ∧
+          lift_rel q3 q4 ∧
+          force_rel NONE q4 q5 ∧
+          proj_rel q5 (exp_of a_exp)` by (
+       qpat_x_assum ‘(∀c z. x = Var c z ⇒ a_exp ≠ Var z) ⇒ _’ mp_tac
        \\ disch_then (assume_tac o ONCE_REWRITE_RULE [IMP_DISJ_THM])
        \\ reverse $ gvs []
-       >- metis_tac [delay_force_Delay]
+       >- (
+        rpt $ goal_assum drule
+        \\ irule_at (Pos hd) thunk_unthunkProofTheory.delay_force_Delay
+        \\ simp [undelay_cases, lift_cases, force_cases, proj_cases,
+                 PULL_EXISTS]
+        \\ rpt $ goal_assum drule)
        \\ fs [exp_of'_def]
-       \\irule_at Any pure_to_thunk_1ProofTheory.compile_rel_Var
-       \\ irule_at Any thunk_case_liftProofTheory.compile_rel_Force
-       \\ irule_at Any thunk_let_forceProofTheory.exp_rel_Force
-       \\ irule_at Any thunk_case_projProofTheory.compile_rel_Force
-       \\ irule_at Any thunk_case_liftProofTheory.compile_rel_Var
-       \\ irule_at Any thunk_let_forceProofTheory.exp_rel_Var
-       \\ irule_at Any thunk_case_projProofTheory.compile_rel_Var
-       \\ irule_at Any thunk_unthunkProofTheory.delay_force_Delat_Force_Var)
+       \\ simp [to_thunk_cases, proj_cases, PULL_EXISTS]
+       \\ irule_at (Pos hd) thunk_unthunkProofTheory.delay_force_Delat_Force_Var
+       \\ simp [undelay_cases, lift_cases, force_cases, proj_cases,
+                PULL_EXISTS])
     \\ qpat_x_assum ‘to_thunk (exp_of' x) _’ $ irule_at Any
+    \\ qpat_x_assum ‘delay_force _ _’ $ irule_at Any
+    \\ qpat_x_assum ‘undelay _ _’ $ irule_at Any
     \\ qpat_x_assum ‘lift_rel _ _’ $ irule_at Any
     \\ qpat_x_assum ‘force_rel NONE _ _’ $ irule_at Any
     \\ qpat_x_assum ‘proj_rel _ _’ $ irule_at Any \\ fs []
@@ -334,28 +326,20 @@ Proof
     \\ PairCases_on ‘h’ \\ fs []
     \\ rename [‘_ = yy :: _’]
     \\ PairCases_on ‘yy’ \\ gvs [rows_of'_def]
-    \\ simp [Once pure_to_thunk_1ProofTheory.compile_rel_cases,PULL_EXISTS]
-    \\ simp [Once pure_to_thunk_1ProofTheory.compile_rel_cases,PULL_EXISTS]
-    \\ simp [Once pure_to_thunk_1ProofTheory.compile_rel_cases,PULL_EXISTS]
+    \\ ntac 3 (simp [to_thunk_cases,PULL_EXISTS])
+    \\ ntac 4 (simp [delay_force_cases, PULL_EXISTS])
+    \\ ntac 4 (simp [undelay_cases, PULL_EXISTS])
     \\ irule_at Any thunk_case_liftProofTheory.compile_rel_Lift
     \\ irule_at Any thunk_case_liftProofTheory.compile_rel_Force
     \\ irule_at Any thunk_case_liftProofTheory.compile_rel_Var
-    \\ fs [freevars_def]
-    \\ irule_at Any thunk_case_projProofTheory.compile_rel_Let_SOME
-    \\ irule_at Any thunk_case_projProofTheory.compile_rel_Force
-    \\ irule_at Any thunk_case_projProofTheory.compile_rel_Var
+    \\ gvs [freevars_def]
     \\ irule_at Any thunk_let_forceProofTheory.exp_rel_Let_Force_Var
-    \\ fs []
-    \\ irule_at Any thunk_let_forceProofTheory.exp_rel_If \\ fs []
-    \\ irule_at Any thunk_let_forceProofTheory.exp_rel_Prim \\ fs [PULL_EXISTS]
+    \\ gvs []
+    \\ ntac 2 (simp [force_cases, PULL_EXISTS])
     \\ irule_at Any thunk_let_forceProofTheory.exp_rel_Force_Var
+    \\ gvs []
+    \\ ntac 3 (simp [proj_cases, PULL_EXISTS])
     \\ fs [rows_of_def]
-    \\ irule_at Any thunk_case_projProofTheory.compile_rel_If \\ fs []
-    \\ irule_at Any thunk_case_projProofTheory.compile_rel_Prim \\ fs []
-    \\ irule_at Any thunk_case_projProofTheory.compile_rel_Var \\ fs []
-    \\ irule_at Any thunk_unthunkProofTheory.delay_force_If \\ fs []
-    \\ irule_at Any thunk_unthunkProofTheory.delay_force_Prim \\ fs []
-    \\ irule_at Any thunk_unthunkProofTheory.delay_force_Var \\ fs []
     \\ drule lets_for_lemma
     \\ rpt $ disch_then drule
     \\ ‘¬MEM (explode fresh) (MAP explode h1)’ by fs [MEM_EQ_MEM_MAP_explode]
@@ -378,111 +362,94 @@ Proof
      (fs [rows_of_def,rows_of'_def]
       \\ Cases_on ‘yopt’ \\ fs []
       \\ Cases_on ‘eopt’ \\ gvs []
-      >-
-       (irule_at Any thunk_unthunkProofTheory.delay_force_Prim \\ fs []
-        \\ irule_at Any thunk_case_projProofTheory.compile_rel_Prim \\ fs []
-        \\ irule_at Any thunk_let_forceProofTheory.exp_rel_Prim \\ fs []
-        \\ irule_at Any thunk_case_liftProofTheory.compile_rel_Prim \\ fs []
-        \\ simp [Once pure_to_thunk_1ProofTheory.compile_rel_cases, freevars_def])
+      >- simp [proj_cases, to_thunk_cases, delay_force_cases, undelay_cases,
+               lift_cases, force_cases, freevars_def, PULL_EXISTS]
       \\ PairCases_on ‘x'’ \\ PairCases_on ‘x''’ \\ gvs []
       \\ fs [IfDisj_def]
-      \\ irule_at Any thunk_unthunkProofTheory.delay_force_If \\ fs []
       \\ irule_at Any thunk_case_projProofTheory.compile_rel_If \\ fs []
       \\ irule_at Any thunk_let_forceProofTheory.exp_rel_If \\ fs []
       \\ irule_at Any thunk_case_liftProofTheory.compile_rel_If \\ fs []
+      \\ irule_at Any thunk_undelay_nextProofTheory.exp_rel_If \\ fs []
+      \\ irule_at Any thunk_unthunkProofTheory.delay_force_If \\ fs []
       \\ irule_at Any pure_to_thunk_1ProofTheory.compile_rel_If \\ fs []
       \\ irule_at Any to_thunk_Disj
       \\ first_assum $ irule_at $ Pos hd
       \\ irule_at Any pure_to_thunk_1ProofTheory.compile_rel_Prim \\ fs []
+      \\ irule_at Any delay_force_Disj
+      \\ irule_at Any undelay_Disj
       \\ irule_at Any lift_rel_Disj
-      \\ first_assum $ irule_at $ Pos hd
-      \\ irule_at Any thunk_case_liftProofTheory.compile_rel_Prim \\ fs []
       \\ irule_at Any force_rel_Disj
-      \\ irule_at Any thunk_let_forceProofTheory.exp_rel_NONE_IMP_SOME
-      \\ first_assum $ irule_at $ Pos hd
-      \\ irule_at Any thunk_let_forceProofTheory.exp_rel_Prim \\ fs []
       \\ irule_at Any proj_rel_Disj
-      \\ fs [freevars_def,SF DNF_ss]
-      \\ first_assum $ irule_at $ Pos hd
-      \\ fs [] \\ imp_res_tac to_thunk_freevars \\ fs []
-      \\ irule_at Any thunk_case_projProofTheory.compile_rel_Prim \\ fs []
+      \\ fs [freevars_def]
       \\ irule_at Any freevars_Disj' \\ fs []
-      \\ irule_at Any thunk_unthunkProofTheory.delay_force_Prim \\ fs []
-      \\ irule_at Any delay_force_Disj)
+      \\ goal_assum drule \\ simp [delay_force_cases]
+      \\ goal_assum drule \\ simp [undelay_cases]
+      \\ goal_assum drule \\ simp [lift_cases]
+      \\ irule_at Any thunk_let_forceProofTheory.exp_rel_NONE_IMP_SOME
+      \\ goal_assum drule \\ simp [force_cases, proj_cases]
+      \\ simp [freevars_def]
+      \\ imp_res_tac to_thunk_freevars \\ fs []
+      \\ imp_res_tac thunk_unthunkProofTheory.delay_force_freevars \\ fs []
+      \\ imp_res_tac thunk_undelay_nextProofTheory.exp_rel_freevars \\ fs [])
     \\ fs [FORALL_PROD]
     \\ rw [] \\ gvs []
     \\ first_x_assum dxrule
     \\ strip_tac
     \\ fs [rows_of_def,rows_of'_def]
-    \\ simp [Once pure_to_thunk_1ProofTheory.compile_rel_cases,PULL_EXISTS]
-    \\ simp [Once pure_to_thunk_1ProofTheory.compile_rel_cases,PULL_EXISTS]
-    \\ simp [Once pure_to_thunk_1ProofTheory.compile_rel_cases,PULL_EXISTS]
+    \\ ntac 3 (simp [to_thunk_cases, PULL_EXISTS])
     \\ fs [freevars_def]
     \\ qpat_x_assum ‘to_thunk _ _’ $ irule_at Any
-    \\ irule_at Any thunk_case_liftProofTheory.compile_rel_If \\ fs [PULL_EXISTS]
-    \\ irule_at Any thunk_case_liftProofTheory.compile_rel_Prim \\ fs [PULL_EXISTS]
-    \\ irule_at Any thunk_case_liftProofTheory.compile_rel_Force
-    \\ irule_at Any thunk_case_liftProofTheory.compile_rel_Var
-    \\ irule_at Any thunk_unthunkProofTheory.delay_force_If \\ fs [PULL_EXISTS]
-    \\ irule_at Any thunk_unthunkProofTheory.delay_force_Prim \\ fs [PULL_EXISTS]
-    \\ irule_at Any thunk_unthunkProofTheory.delay_force_Var
-    \\ irule_at Any thunk_case_projProofTheory.compile_rel_If \\ fs [PULL_EXISTS]
-    \\ irule_at Any thunk_case_projProofTheory.compile_rel_Prim \\ fs [PULL_EXISTS]
-    \\ irule_at Any thunk_case_projProofTheory.compile_rel_Var
-    \\ simp [Once thunk_let_forceProofTheory.exp_rel_cases]
-    \\ simp [Once thunk_let_forceProofTheory.exp_rel_cases]
-    \\ simp [Once thunk_let_forceProofTheory.exp_rel_cases]
+    \\ ntac 4 (simp [delay_force_cases, PULL_EXISTS])
+    \\ ntac 4 (simp [undelay_cases, PULL_EXISTS])
+    \\ fs [freevars_def]
+    \\ irule_at Any thunk_case_liftProofTheory.compile_rel_If
+    \\ fs [PULL_EXISTS]
+    \\ ntac 3 (simp [lift_cases, PULL_EXISTS])
+    \\ ntac 2 (simp [force_cases, PULL_EXISTS])
+    \\ irule_at Any thunk_let_forceProofTheory.exp_rel_Force_Var
+    \\ ntac 3 (simp [proj_cases, PULL_EXISTS])
     \\ drule lets_for_lemma
-    \\ ntac 4 $ disch_then drule
+    \\ ntac 5 (disch_then drule)
     \\ disch_then $ drule_at $ Pos last
     \\ rename [‘lets_for' (LENGTH cs) (explode cn)’]
     \\ disch_then $ qspecl_then [‘explode v’,
             ‘explode cn’,‘MAP explode cs’,‘0’] mp_tac
     \\ impl_tac >- fs [GSYM MEM_EQ_MEM_MAP_explode]
     \\ fs [] \\ strip_tac
-    \\ rpt $ pop_assum $ irule_at Any
-    \\ first_assum $ irule_at Any
-    \\ first_assum $ irule_at Any
-    \\ fs [])
-  >~ [‘Seq’] >-
-   (fs [pure_cexpTheory.op_of_def]
-    \\ irule_at Any pure_to_thunk_1ProofTheory.compile_rel_Seq_fresh \\ fs []
-    \\ qpat_x_assum ‘explode fresh ∉ _’ $ irule_at Any
-    \\ irule_at Any thunk_case_liftProofTheory.compile_rel_Let
-    \\ irule_at Any thunk_let_forceProofTheory.exp_rel_Let
-    \\ fs [name_clash_def]
-    \\ irule_at Any thunk_case_projProofTheory.compile_rel_Let_SOME
+    \\ rpt $ pop_assum $ irule_at Any)
+  >~ [‘Seq’] >- (
+   fs [pure_cexpTheory.op_of_def]
+   \\ irule_at Any pure_to_thunk_1ProofTheory.compile_rel_Seq_fresh \\ fs []
+   \\ rpt $ goal_assum drule
+   \\ irule_at Any thunk_unthunkProofTheory.delay_force_Let_fresh
+   \\ rpt $ goal_assum drule
+   \\ imp_res_tac pure_to_thunk_1ProofTheory.compile_rel_freevars \\ gvs []
+   \\ simp [undelay_cases, lift_cases, proj_cases, PULL_EXISTS]
+   \\ rpt $ goal_assum drule
+   \\ irule_at Any thunk_let_forceProofTheory.exp_rel_Let \\ fs []
+   \\ rpt $ goal_assum drule)
+  >~ [‘Let’] >- (
+    irule_at Any pure_to_thunk_1ProofTheory.compile_rel_Let
+    \\ rpt $ goal_assum drule
     \\ irule_at Any thunk_unthunkProofTheory.delay_force_Let
-    \\ metis_tac [])
-  >~ [‘Let’] >-
-   (irule_at Any pure_to_thunk_1ProofTheory.compile_rel_Let
-    \\ irule_at Any thunk_case_liftProofTheory.compile_rel_Let
-    \\ irule_at Any thunk_let_forceProofTheory.exp_rel_Let
-    \\ fs [name_clash_def]
-    \\ irule_at Any thunk_case_projProofTheory.compile_rel_Let_SOME
-    \\ irule_at Any thunk_unthunkProofTheory.delay_force_Let
-    \\ irule_at Any thunk_case_liftProofTheory.compile_rel_Delay
-    \\ irule_at Any thunk_let_forceProofTheory.exp_rel_Delay
-    \\ irule_at Any thunk_case_projProofTheory.compile_rel_Delay
-    \\ gvs [IMP_DISJ_THM,exp_of'_def]
-    >-
-     (irule_at Any pure_to_thunk_1ProofTheory.compile_rel_Var
-      \\ irule_at Any thunk_case_liftProofTheory.compile_rel_Force
-      \\ irule_at Any thunk_let_forceProofTheory.exp_rel_Force
-      \\ irule_at Any thunk_case_projProofTheory.compile_rel_Force
-      \\ irule_at Any thunk_case_liftProofTheory.compile_rel_Var
-      \\ irule_at Any thunk_let_forceProofTheory.exp_rel_Var
-      \\ irule_at Any thunk_case_projProofTheory.compile_rel_Var
+    \\ simp [undelay_cases, lift_cases, proj_cases, PULL_EXISTS]
+    \\ irule_at Any thunk_let_forceProofTheory.exp_rel_Let \\ simp []
+    \\ gvs [IMP_DISJ_THM, exp_of'_def]
+    >- (
+      simp [to_thunk_cases, PULL_EXISTS]
       \\ irule_at Any thunk_unthunkProofTheory.delay_force_Delat_Force_Var
-      \\ metis_tac [])
-    \\ irule_at Any thunk_unthunkProofTheory.delay_force_Delay
+      \\ simp [undelay_cases, lift_cases, proj_cases, force_cases, PULL_EXISTS]
+      \\ rpt $ goal_assum drule)
+    \\ simp [proj_cases, force_cases, lift_cases, undelay_cases,
+             delay_force_cases, PULL_EXISTS]
     \\ metis_tac [])
-  >~ [‘Cons _ _’] >-
-   (irule_at Any pure_to_thunk_1ProofTheory.compile_rel_Cons
+  >~ [‘Cons _ _’] >- (
+    irule_at Any pure_to_thunk_1ProofTheory.compile_rel_Cons
+    \\ irule_at Any thunk_unthunkProofTheory.delay_force_Prim
+    \\ irule_at Any thunk_undelay_nextProofTheory.exp_rel_Prim
     \\ irule_at Any thunk_case_liftProofTheory.compile_rel_Prim
     \\ irule_at Any thunk_let_forceProofTheory.exp_rel_Prim
-    \\ irule_at Any thunk_case_projProofTheory.compile_rel_Cons
-    \\ irule_at Any thunk_unthunkProofTheory.delay_force_Prim
+    \\ irule_at Any thunk_case_projProofTheory.compile_rel_Prim
     \\ fs []
     \\ pop_assum mp_tac
     \\ pop_assum kall_tac
@@ -500,37 +467,29 @@ Proof
     \\ qpat_x_assum ‘(∀c z. h = Var c z ⇒ h5 ≠ Var z) ⇒ _’ mp_tac
     \\ disch_then (assume_tac o ONCE_REWRITE_RULE [IMP_DISJ_THM])
     \\ reverse $ gvs []
-    >-
-     (qpat_x_assum ‘to_thunk (exp_of' _) _’ $ irule_at Any
-      \\ irule_at Any thunk_case_liftProofTheory.compile_rel_Delay
-      \\ qpat_x_assum ‘lift_rel y1 _’ $ irule_at Any
+    >- (
+      irule_at Any thunk_case_projProofTheory.compile_rel_Delay
       \\ irule_at Any thunk_let_forceProofTheory.exp_rel_Delay
-      \\ qpat_x_assum ‘force_rel NONE y2 _’ $ irule_at Any
-      \\ irule_at Any thunk_case_projProofTheory.compile_rel_Delay
-      \\ first_x_assum $ irule_at $ Pos hd
-      \\ fs []
-      \\ irule_at Any thunk_unthunkProofTheory.delay_force_Delay \\ fs [])
-    \\ fs [cexp_wf_def,SF SFY_ss,exp_of'_def]
+      \\ irule_at Any thunk_case_liftProofTheory.compile_rel_Delay
+      \\ irule_at Any thunk_undelay_nextProofTheory.exp_rel_Delay
+      \\ irule_at Any thunk_unthunkProofTheory.delay_force_Delay
+      \\ metis_tac [])
+    \\ gvs [cexp_wf_def, SF SFY_ss, exp_of'_def]
     \\ irule_at Any pure_to_thunk_1ProofTheory.compile_rel_Var
-    \\ irule_at Any thunk_case_liftProofTheory.compile_rel_Delay
-    \\ irule_at Any thunk_case_liftProofTheory.compile_rel_Force
-    \\ irule_at Any thunk_case_liftProofTheory.compile_rel_Var
-    \\ irule_at Any thunk_let_forceProofTheory.exp_rel_Delay
-    \\ irule_at Any thunk_let_forceProofTheory.exp_rel_Force
-    \\ irule_at Any thunk_let_forceProofTheory.exp_rel_Var
-    \\ irule_at Any thunk_case_projProofTheory.compile_rel_Delay
-    \\ irule_at Any thunk_case_projProofTheory.compile_rel_Force
-    \\ irule_at Any thunk_case_projProofTheory.compile_rel_Var
     \\ irule_at Any thunk_unthunkProofTheory.delay_force_Delat_Force_Var
-    \\ fs [])
-  >~ [‘Apps’] >-
-   (pop_assum kall_tac
+    \\ irule_at Any thunk_undelay_nextProofTheory.exp_rel_Var
+    \\ irule_at Any thunk_case_liftProofTheory.compile_rel_Var
+    \\ irule_at Any thunk_let_forceProofTheory.exp_rel_Var
+    \\ irule_at Any thunk_case_projProofTheory.compile_rel_Var)
+  >~ [‘Apps’] >- (
+    pop_assum kall_tac
     \\ rpt $ pop_assum mp_tac
     \\ qid_spec_tac ‘x’
     \\ qid_spec_tac ‘y1’
     \\ qid_spec_tac ‘y2’
     \\ qid_spec_tac ‘y3’
     \\ qid_spec_tac ‘y4’
+    \\ qid_spec_tac ‘y5’
     \\ qid_spec_tac ‘y’
     \\ qid_spec_tac ‘ys’
     \\ qid_spec_tac ‘xs’
@@ -552,48 +511,37 @@ Proof
     \\ disch_then irule
     \\ irule_at Any pure_to_thunk_1ProofTheory.compile_rel_App
     \\ qpat_x_assum ‘to_thunk (exp_of' _) _’ $ irule_at Any
+    \\ irule_at Any thunk_unthunkProofTheory.delay_force_App
+    \\ irule_at Any thunk_undelay_nextProofTheory.exp_rel_App
     \\ irule_at Any thunk_case_liftProofTheory.compile_rel_App
     \\ irule_at Any thunk_let_forceProofTheory.exp_rel_App
     \\ irule_at Any thunk_case_projProofTheory.compile_rel_App
-    \\ irule_at Any thunk_unthunkProofTheory.delay_force_App
     \\ qpat_x_assum ‘LIST_REL _ _ _’ kall_tac
     \\ qpat_x_assum ‘(∀c z. h = Var c z ⇒ h5 ≠ Var z) ⇒ _’ mp_tac
     \\ disch_then (assume_tac o ONCE_REWRITE_RULE [IMP_DISJ_THM])
     \\ reverse $ gvs []
-    >-
-     (qpat_x_assum ‘to_thunk (exp_of' _) _’ $ irule_at Any
-      \\ qpat_x_assum ‘lift_rel y1 _’ $ irule_at Any
-      \\ qpat_x_assum ‘force_rel NONE y2 _’ $ irule_at Any
-      \\ first_x_assum $ irule_at $ Pos hd
-      \\ irule_at Any thunk_unthunkProofTheory.delay_force_Delay
-      \\ irule_at Any thunk_case_liftProofTheory.compile_rel_Delay
-      \\ first_x_assum $ irule_at $ Pos hd
-      \\ first_x_assum $ irule_at $ Pos hd \\ fs []
-      \\ irule_at Any thunk_case_projProofTheory.compile_rel_Delay
-      \\ first_x_assum $ irule_at $ Pos hd \\ fs []
-      \\ irule_at Any thunk_let_forceProofTheory.exp_rel_Delay
-      \\ fs [cexp_wf_def,SF SFY_ss])
-    \\ first_x_assum $ irule_at $ Pos hd
-    \\ fs [cexp_wf_def,SF SFY_ss,exp_of'_def]
-    \\ qpat_x_assum ‘proj_rel _ y4’ $ irule_at Any
-    \\ qpat_x_assum ‘lift_rel y1 _’ $ irule_at Any \\ gvs []
-    \\ irule_at Any pure_to_thunk_1ProofTheory.compile_rel_Var
-    \\ irule_at Any thunk_case_liftProofTheory.compile_rel_Delay
-    \\ irule_at Any thunk_case_liftProofTheory.compile_rel_Force
-    \\ irule_at Any thunk_case_liftProofTheory.compile_rel_Var
-    \\ irule_at Any thunk_let_forceProofTheory.exp_rel_Delay
-    \\ irule_at Any thunk_let_forceProofTheory.exp_rel_Force
-    \\ irule_at Any thunk_let_forceProofTheory.exp_rel_Var
-    \\ irule_at Any thunk_case_projProofTheory.compile_rel_Delay
-    \\ irule_at Any thunk_case_projProofTheory.compile_rel_Force
-    \\ irule_at Any thunk_case_projProofTheory.compile_rel_Var
-    \\ irule_at Any thunk_unthunkProofTheory.delay_force_Delat_Force_Var)
-  >~ [‘AtomOp’] >-
-   (irule_at Any pure_to_thunk_1ProofTheory.compile_rel_Prim \\ fs []
+    >- (
+      qpat_x_assum ‘to_thunk (exp_of' _) _’ $ irule_at Any
+      \\ goal_assum drule \\ simp [proj_cases, PULL_EXISTS]
+      \\ ntac 2 (goal_assum drule) \\ simp [force_cases, PULL_EXISTS]
+      \\ ntac 2 (goal_assum drule) \\ simp [lift_cases, PULL_EXISTS]
+      \\ ntac 2 (goal_assum drule) \\ simp [undelay_cases, PULL_EXISTS]
+      \\ goal_assum drule \\ simp [delay_force_cases, PULL_EXISTS]
+      \\ fs [cexp_wf_def])
+    \\ goal_assum drule \\ simp [proj_cases, PULL_EXISTS]
+    \\ goal_assum drule \\ simp [force_cases, PULL_EXISTS]
+    \\ goal_assum drule \\ simp [lift_cases, PULL_EXISTS]
+    \\ goal_assum drule \\ simp [undelay_cases, PULL_EXISTS]
+    \\ simp [delay_force_cases, PULL_EXISTS]
+    \\ simp [exp_of'_def, to_thunk_cases, PULL_EXISTS]
+    \\ simp [cexp_wf_def])
+  >~ [‘AtomOp’] >- (
+    irule_at Any pure_to_thunk_1ProofTheory.compile_rel_Prim \\ fs []
+    \\ irule_at Any thunk_unthunkProofTheory.delay_force_Prim
+    \\ irule_at Any thunk_undelay_nextProofTheory.exp_rel_Prim
     \\ irule_at Any thunk_case_liftProofTheory.compile_rel_Prim
     \\ irule_at Any thunk_let_forceProofTheory.exp_rel_Prim
     \\ irule_at Any thunk_case_projProofTheory.compile_rel_Prim \\ fs []
-    \\ irule_at Any thunk_unthunkProofTheory.delay_force_Prim \\ fs []
     \\ pop_assum kall_tac
     \\ pop_assum kall_tac
     \\ pop_assum mp_tac
@@ -605,22 +553,24 @@ Proof
     \\ rw [] \\ gvs []
     \\ last_x_assum drule \\ strip_tac
     \\ rpt $ first_assum $ irule_at Any)
-  >~ [‘Lams’] >-
-   (qpat_x_assum ‘_ ≠ []’ kall_tac
+  >~ [‘Lams’] >- (
+    qpat_x_assum ‘_ ≠ []’ kall_tac
     \\ qid_spec_tac ‘s’ \\ Induct \\ fs [pure_expTheory.Lams_def]
     >- (rpt $ first_assum $ irule_at Any)
     \\ rw []
     \\ irule_at Any pure_to_thunk_1ProofTheory.compile_rel_Lam \\ fs []
-    \\ irule_at Any thunk_unthunkProofTheory.delay_force_Lam \\ fs []
+    \\ irule_at Any thunk_unthunkProofTheory.delay_force_Lam
+    \\ irule_at Any thunk_undelay_nextProofTheory.exp_rel_Lam
     \\ irule_at Any thunk_case_projProofTheory.compile_rel_Lam \\ fs []
     \\ irule_at Any thunk_case_liftProofTheory.compile_rel_Lam
     \\ irule_at Any thunk_let_forceProofTheory.exp_rel_Lam \\ fs []
     \\ rpt $ first_assum $ irule_at Any)
-  >~ [‘Letrec’] >-
-   (qpat_x_assum ‘_ ≠ []’ kall_tac
+  >~ [‘Letrec’] >- (
+    qpat_x_assum ‘_ ≠ []’ kall_tac
     \\ irule_at Any pure_to_thunk_1ProofTheory.compile_rel_Letrec \\ fs []
+    \\ irule_at Any thunk_unthunkProofTheory.delay_force_Letrec
+    \\ irule_at Any thunk_undelay_nextProofTheory.exp_rel_Letrec
     \\ irule_at Any thunk_case_projProofTheory.compile_rel_Letrec \\ fs []
-    \\ irule_at Any thunk_unthunkProofTheory.delay_force_Letrec \\ fs []
     \\ irule_at Any thunk_case_liftProofTheory.compile_rel_Letrec
     \\ irule_at Any thunk_let_forceProofTheory.exp_rel_Letrec \\ fs []
     \\ rpt $ first_assum $ irule_at Any
@@ -640,129 +590,160 @@ Proof
     \\ gvs []
     \\ irule_at Any thunk_case_liftProofTheory.compile_rel_Delay
     \\ irule_at Any thunk_unthunkProofTheory.delay_force_Delay
+    \\ irule_at Any thunk_undelay_nextProofTheory.exp_rel_Delay
     \\ irule_at Any thunk_case_projProofTheory.compile_rel_Delay
     \\ irule_at Any thunk_let_forceProofTheory.exp_rel_Delay
     \\ rpt $ first_assum $ irule_at Any
-    \\ EVAL_TAC \\ fs []) >>
-  gvs[num_args_ok_def, pure_configTheory.num_monad_args_def] >>
-  gvs[LENGTH_EQ_NUM_compute] >>
-  simp[to_thunk_cases, PULL_EXISTS, pure_configTheory.monad_cns_def,
-       mop_rel_cases, mop_ret_rel_cases, mop_delay_rel_cases]
-  >~ [`Ret`]
-  >- (
-    simp[lift_cases, force_cases, proj_cases, delay_force_cases, PULL_EXISTS] >>
-    last_x_assum $ mp_tac o ONCE_REWRITE_RULE [IMP_DISJ_THM] >> rw[] >> gvs[]
+    \\ EVAL_TAC \\ fs [])
+  \\ gvs [num_args_ok_def, pure_configTheory.num_monad_args_def]
+  \\ gvs[LENGTH_EQ_NUM_compute]
+  \\ simp[to_thunk_cases, PULL_EXISTS, pure_configTheory.monad_cns_def,
+          mop_rel_cases, mop_ret_rel_cases, mop_delay_rel_cases]
+  >~ [`Ret`] >- (
+    simp [proj_cases, delay_force_cases, force_cases, undelay_cases, lift_cases,
+          PULL_EXISTS]
+    \\ last_x_assum $ mp_tac o ONCE_REWRITE_RULE [IMP_DISJ_THM] \\ rw []
+    \\ gvs []
     >- (
-      simp[exp_of'_def, to_thunk_cases, PULL_EXISTS] >>
-      ntac 3 $ simp[lift_cases, force_cases, proj_cases, delay_force_cases, PULL_EXISTS]
-      ) >>
-    simp[lift_cases, force_cases, proj_cases, delay_force_cases, PULL_EXISTS] >>
-    rpt $ goal_assum drule
-    )
-  >~ [`Raise`]
-  >- (
-    simp[lift_cases, force_cases, proj_cases, delay_force_cases, PULL_EXISTS] >>
-    last_x_assum $ mp_tac o ONCE_REWRITE_RULE [IMP_DISJ_THM] >> rw[] >> gvs[]
+      simp [exp_of'_def, to_thunk_cases, PULL_EXISTS]
+      \\ irule_at Any thunk_unthunkProofTheory.delay_force_Delat_Force_Var
+      \\ simp [undelay_cases, lift_cases, proj_cases, force_cases, PULL_EXISTS])
+    \\ simp [proj_cases, force_cases, lift_cases, undelay_cases,
+             delay_force_cases, PULL_EXISTS]
+    \\ rpt $ goal_assum drule)
+  >~ [`Raise`] >- (
+    simp [proj_cases, delay_force_cases, force_cases, undelay_cases, lift_cases,
+          PULL_EXISTS]
+    \\ last_x_assum $ mp_tac o ONCE_REWRITE_RULE [IMP_DISJ_THM] \\ rw []
+    \\ gvs []
     >- (
-      simp[exp_of'_def, to_thunk_cases, PULL_EXISTS] >>
-      ntac 3 $ simp[lift_cases, force_cases, proj_cases, delay_force_cases, PULL_EXISTS]
-      ) >>
-    simp[lift_cases, force_cases, proj_cases, delay_force_cases, PULL_EXISTS] >>
-    rpt $ goal_assum drule
-    )
-  >~ [`Bind`]
-  >- (
-    simp[lift_cases, force_cases, proj_cases, delay_force_cases, PULL_EXISTS] >>
-    rpt $ goal_assum drule
-    )
-  >~ [`Handle`]
-  >- (
-    simp[lift_cases, force_cases, proj_cases, delay_force_cases, PULL_EXISTS] >>
-    rpt $ goal_assum $ drule
-    )
-  >~ [`Act`]
-  >- (
-    simp[lift_cases, force_cases, proj_cases, delay_force_cases, PULL_EXISTS] >>
-    goal_assum drule >> simp[lift_cases, PULL_EXISTS] >>
-    goal_assum drule >> ntac 4 $ simp[lift_cases, PULL_EXISTS] >>
-    simp[force_cases, PULL_EXISTS] >> goal_assum drule >>
-    ntac 4 $ simp[force_cases, PULL_EXISTS] >>
-    simp[proj_cases, PULL_EXISTS] >> goal_assum drule >>
-    ntac 4 $ simp[proj_cases, PULL_EXISTS] >>
-    ntac 5 $ simp[delay_force_cases]
-    )
-  >~ [`Length`]
-  >- (
-    simp[lift_cases, force_cases, proj_cases, delay_force_cases, PULL_EXISTS] >>
-    goal_assum drule >> simp[lift_cases, PULL_EXISTS] >>
-    goal_assum drule >> ntac 4 $ simp[lift_cases, PULL_EXISTS] >>
-    simp[force_cases, PULL_EXISTS] >> goal_assum drule >>
-    ntac 4 $ simp[force_cases, PULL_EXISTS] >>
-    simp[proj_cases, PULL_EXISTS] >> goal_assum drule >>
-    ntac 4 $ simp[proj_cases, PULL_EXISTS] >>
-    ntac 5 $ simp[delay_force_cases]
-    )
-  >~ [`Alloc`] (* Delay (Force (Var _)) case *)
-  >- (
-    simp[lift_cases, force_cases, proj_cases, delay_force_cases, PULL_EXISTS] >>
-    goal_assum drule >> simp[exp_of'_def, to_thunk_cases, PULL_EXISTS] >>
-    simp[LUPDATE_DEF] >> simp[lift_cases, PULL_EXISTS] >> goal_assum drule >>
-    ntac 7 $ simp[lift_cases, PULL_EXISTS] >> simp[force_cases, PULL_EXISTS] >>
-    goal_assum drule >> ntac 7 $ simp[force_cases, PULL_EXISTS] >>
-    simp[proj_cases, PULL_EXISTS] >> goal_assum drule >>
-    ntac 7 $ simp[proj_cases, PULL_EXISTS] >> ntac 6 $ simp[delay_force_cases]
-    )
-  >~ [`Alloc`]
-  >- (
-    simp[LUPDATE_DEF] >>
-    ntac 2 $ simp[lift_cases, PULL_EXISTS] >> rpt $ goal_assum drule >>
-    simp[lift_cases, PULL_EXISTS] >> goal_assum drule >>
-    ntac 7 $ simp[lift_cases, PULL_EXISTS] >>
-    ntac 2 $ simp[force_cases, PULL_EXISTS] >> goal_assum drule >>
-    simp[force_cases, PULL_EXISTS] >> goal_assum drule >>
-    ntac 7 $ simp[force_cases, PULL_EXISTS] >>
-    ntac 2 $ simp[proj_cases, PULL_EXISTS] >> goal_assum drule >>
-    simp[proj_cases, PULL_EXISTS] >> goal_assum drule >>
-    ntac 7 $ simp[proj_cases, PULL_EXISTS] >>
-    ntac 7 $ simp[delay_force_cases, PULL_EXISTS]
-    )
-  >~ [`Deref`]
-  >- (
-    ntac 2 $ simp[lift_cases, PULL_EXISTS] >> rpt $ goal_assum drule >>
-    ntac 4 $ simp[lift_cases, PULL_EXISTS] >>
-    ntac 2 $ simp[force_cases, PULL_EXISTS] >> rpt $ goal_assum drule >>
-    ntac 4 $ simp[force_cases, PULL_EXISTS] >>
-    ntac 2 $ simp[proj_cases, PULL_EXISTS] >> rpt $ goal_assum drule >>
-    ntac 4 $ simp[proj_cases, PULL_EXISTS] >>
-    ntac 2 $ simp[delay_force_cases, PULL_EXISTS] >> rpt $ goal_assum drule >>
-    ntac 4 $ simp[delay_force_cases, PULL_EXISTS]
-    )
-  >~ [`Update`] (* Delay (Force (Var _)) case *)
-  >- (
-    simp[LUPDATE_DEF, exp_of'_def] >> rpt $ goal_assum drule >>
-    simp[to_thunk_cases, PULL_EXISTS] >>
-    ntac 3 $ simp[lift_cases, PULL_EXISTS] >> rpt $ goal_assum drule >>
-    ntac 11 $ simp[lift_cases, PULL_EXISTS] >>
-    ntac 3 $ simp[force_cases, PULL_EXISTS] >> rpt $ goal_assum drule >>
-    ntac 11 $ simp[force_cases, PULL_EXISTS] >>
-    ntac 3 $ simp[proj_cases, PULL_EXISTS] >> rpt $ goal_assum drule >>
-    ntac 11 $ simp[proj_cases, PULL_EXISTS] >>
-    ntac 12 $ simp[Once delay_force_cases]
-    )
-  >~ [`Update`]
-  >- (
-    simp[LUPDATE_DEF, exp_of'_def] >> rpt $ goal_assum drule >>
-    ntac 3 $ simp[lift_cases, PULL_EXISTS] >> rpt $ goal_assum drule >>
-    simp[lift_cases, PULL_EXISTS] >> goal_assum drule >>
-    ntac 11 $ simp[lift_cases, PULL_EXISTS] >>
-    ntac 3 $ simp[force_cases, PULL_EXISTS] >> rpt $ goal_assum drule >>
-    simp[force_cases, PULL_EXISTS] >> goal_assum drule >>
-    ntac 11 $ simp[force_cases, PULL_EXISTS] >>
-    ntac 3 $ simp[proj_cases, PULL_EXISTS] >> rpt $ goal_assum drule >>
-    simp[proj_cases, PULL_EXISTS] >> goal_assum drule >>
-    ntac 11 $ simp[proj_cases, PULL_EXISTS] >>
-    ntac 12 $ simp[Once delay_force_cases]
-    )
+      simp [exp_of'_def, to_thunk_cases, PULL_EXISTS]
+      \\ irule_at Any thunk_unthunkProofTheory.delay_force_Delat_Force_Var
+      \\ simp [undelay_cases, lift_cases, force_cases, proj_cases, PULL_EXISTS])
+    \\ simp [proj_cases, force_cases, lift_cases, undelay_cases,
+             delay_force_cases, PULL_EXISTS]
+    \\ rpt $ goal_assum drule)
+  >~ [`Bind`] >- (
+    simp [proj_cases, force_cases, lift_cases, delay_force_cases,
+          undelay_cases, PULL_EXISTS]
+    \\ rpt $ goal_assum drule)
+  >~ [`Handle`] >- (
+    simp [proj_cases, force_cases, lift_cases, delay_force_cases,
+          undelay_cases, PULL_EXISTS]
+    \\ rpt $ goal_assum drule)
+  >~ [`Act`] >- (
+    irule_at Any thunk_case_projProofTheory.compile_rel_Monad
+    \\ irule_at Any thunk_let_forceProofTheory.exp_rel_Monad
+    \\ irule_at Any thunk_case_liftProofTheory.compile_rel_Monad
+    \\ irule_at Any thunk_unthunkProofTheory.delay_force_Monad
+    \\ irule_at Any thunk_undelay_nextProofTheory.exp_rel_Monad_Ret_Delay
+    \\ simp [PULL_EXISTS]
+    \\ irule_at Any thunk_case_liftProofTheory.compile_rel_Monad
+    \\ irule_at Any thunk_case_liftProofTheory.compile_rel_Lam
+    \\ irule_at Any thunk_let_forceProofTheory.exp_rel_Monad
+    \\ irule_at Any thunk_let_forceProofTheory.exp_rel_Lam
+    \\ irule_at Any thunk_case_liftProofTheory.compile_rel_Monad
+    \\ irule_at Any thunk_case_projProofTheory.compile_rel_Monad
+    \\ irule_at Any thunk_case_projProofTheory.compile_rel_Lam
+    \\ irule_at Any thunk_case_projProofTheory.compile_rel_Monad
+    \\ simp [PULL_EXISTS]
+    \\ irule_at Any thunk_case_projProofTheory.compile_rel_Delay
+    \\ irule_at Any thunk_case_projProofTheory.compile_rel_Var
+    \\ irule_at Any thunk_case_liftProofTheory.compile_rel_Delay
+    \\ irule_at Any thunk_case_liftProofTheory.compile_rel_Var
+    \\ irule_at Any thunk_let_forceProofTheory.exp_rel_Monad
+    \\ simp []
+    \\ irule_at Any thunk_let_forceProofTheory.exp_rel_Delay
+    \\ irule_at Any thunk_let_forceProofTheory.exp_rel_Var
+    \\ rpt $ goal_assum drule)
+  >~ [`Length`] >- (
+    irule_at Any thunk_case_projProofTheory.compile_rel_Monad
+    \\ irule_at Any thunk_let_forceProofTheory.exp_rel_Monad
+    \\ irule_at Any thunk_case_liftProofTheory.compile_rel_Monad
+    \\ irule_at Any thunk_unthunkProofTheory.delay_force_Monad
+    \\ irule_at Any thunk_undelay_nextProofTheory.exp_rel_Monad_Ret_Delay
+    \\ simp [PULL_EXISTS]
+    \\ irule_at Any thunk_case_liftProofTheory.compile_rel_Monad
+    \\ irule_at Any thunk_case_liftProofTheory.compile_rel_Lam
+    \\ irule_at Any thunk_let_forceProofTheory.exp_rel_Monad
+    \\ irule_at Any thunk_let_forceProofTheory.exp_rel_Lam
+    \\ irule_at Any thunk_case_liftProofTheory.compile_rel_Monad
+    \\ irule_at Any thunk_case_projProofTheory.compile_rel_Monad
+    \\ irule_at Any thunk_case_projProofTheory.compile_rel_Lam
+    \\ irule_at Any thunk_case_projProofTheory.compile_rel_Monad
+    \\ simp [PULL_EXISTS]
+    \\ irule_at Any thunk_case_projProofTheory.compile_rel_Delay
+    \\ irule_at Any thunk_case_projProofTheory.compile_rel_Var
+    \\ irule_at Any thunk_case_liftProofTheory.compile_rel_Delay
+    \\ irule_at Any thunk_case_liftProofTheory.compile_rel_Var
+    \\ irule_at Any thunk_let_forceProofTheory.exp_rel_Monad
+    \\ simp []
+    \\ irule_at Any thunk_let_forceProofTheory.exp_rel_Delay
+    \\ irule_at Any thunk_let_forceProofTheory.exp_rel_Var
+    \\ rpt $ goal_assum drule)
+  >~ [`Alloc`] >- (
+    (* Delay (Force (Var _)) case *)
+    goal_assum drule
+    \\ simp [exp_of'_def, to_thunk_cases, delay_force_cases, PULL_EXISTS]
+    \\ simp [undelay_cases, PULL_EXISTS]
+    \\ ntac 6 (simp [lift_cases, PULL_EXISTS])
+    \\ ntac 6 (simp [force_cases, PULL_EXISTS])
+    \\ ntac 2 (simp [proj_cases, PULL_EXISTS])
+    \\ simp [LUPDATE_DEF, PULL_EXISTS]
+    \\ goal_assum drule
+    \\ irule_at (Pos hd) thunk_unthunkProofTheory.delay_force_Delat_Force_Var
+    \\ goal_assum drule \\ simp [undelay_cases, PULL_EXISTS]
+    \\ goal_assum drule \\ simp [lift_cases, PULL_EXISTS]
+    \\ goal_assum drule \\ simp [force_cases, PULL_EXISTS]
+    \\ ntac 5 (simp [proj_cases, PULL_EXISTS]))
+  >~ [`Alloc`] >- (
+    ntac 2 (goal_assum drule)
+    \\ simp [delay_force_cases, undelay_cases, PULL_EXISTS]
+    \\ ntac 6 (simp [lift_cases, PULL_EXISTS])
+    \\ ntac 6 (simp [force_cases, PULL_EXISTS])
+    \\ ntac 2 (simp [proj_cases, PULL_EXISTS])
+    \\ simp [LUPDATE_DEF, PULL_EXISTS]
+    \\ goal_assum drule
+    \\ irule_at (Pos hd) thunk_unthunkProofTheory.delay_force_Delay
+    \\ ntac 2 (goal_assum drule) \\ simp [undelay_cases, PULL_EXISTS]
+    \\ ntac 2 (goal_assum drule) \\ simp [lift_cases, PULL_EXISTS]
+    \\ ntac 2 (goal_assum drule) \\ simp [force_cases, PULL_EXISTS]
+    \\ goal_assum drule \\ ntac 5 (simp [proj_cases, PULL_EXISTS]))
+  >~ [`Deref`] >- (
+    ntac 2 (goal_assum drule) \\ simp [delay_force_cases, PULL_EXISTS]
+    \\ ntac 2 (goal_assum drule) \\ simp [undelay_cases, PULL_EXISTS]
+    \\ ntac 2 (goal_assum drule) \\ ntac 2 (simp [lift_cases, PULL_EXISTS])
+    \\ ntac 2 (goal_assum drule) \\ ntac 4 (simp [lift_cases, PULL_EXISTS])
+    \\ ntac 2 (simp [force_cases, PULL_EXISTS]) \\ ntac 2 (goal_assum drule)
+    \\ ntac 4 (simp [force_cases, PULL_EXISTS])
+    \\ ntac 6 (simp [proj_cases, PULL_EXISTS]))
+  >~ [`Update`] >- (
+    (* Delay (Force (Var _)) case *)
+    ntac 2 (goal_assum drule) \\ simp [exp_of'_def, to_thunk_cases, PULL_EXISTS]
+    \\ simp [delay_force_cases, undelay_cases, PULL_EXISTS]
+    \\ ntac 11 (simp [lift_cases, PULL_EXISTS])
+    \\ ntac 11 (simp [force_cases, PULL_EXISTS])
+    \\ ntac 3 (simp [proj_cases, PULL_EXISTS])
+    \\ simp [LUPDATE_DEF, PULL_EXISTS]
+    \\ ntac 2 (goal_assum drule)
+    \\ irule_at (Pos hd) thunk_unthunkProofTheory.delay_force_Delat_Force_Var
+    \\ ntac 2 (goal_assum drule) \\ simp [undelay_cases, PULL_EXISTS]
+    \\ ntac 2 (goal_assum drule) \\ simp [lift_cases, PULL_EXISTS]
+    \\ ntac 2 (goal_assum drule) \\ simp [force_cases, PULL_EXISTS]
+    \\ ntac 9 (simp [proj_cases, PULL_EXISTS]))
+  >~ [`Update`] >- (
+    ntac 3 (goal_assum drule)
+    \\ simp [delay_force_cases, undelay_cases, PULL_EXISTS]
+    \\ ntac 11 (simp [lift_cases, PULL_EXISTS])
+    \\ ntac 11 (simp [force_cases, PULL_EXISTS])
+    \\ ntac 3 (simp [proj_cases, PULL_EXISTS])
+    \\ simp [LUPDATE_DEF, PULL_EXISTS]
+    \\ ntac 2 (goal_assum drule)
+    \\ irule_at (Pos hd) thunk_unthunkProofTheory.delay_force_Delay
+    \\ ntac 3 (goal_assum drule) \\ simp [undelay_cases, PULL_EXISTS]
+    \\ ntac 3 (goal_assum drule) \\ simp [lift_cases, PULL_EXISTS]
+    \\ ntac 3 (goal_assum drule) \\ simp [force_cases, PULL_EXISTS]
+    \\ goal_assum drule \\ ntac 9 (simp [proj_cases, PULL_EXISTS]))
 QED
 
 Theorem exp_rel_semantics:
@@ -783,26 +764,21 @@ Proof
      \\ irule_at Any pure_obs_sem_equalTheory.bisimilarity_IMP_semantics_eq
      \\ fs [pure_exp_relTheory.app_bisimilarity_eq])
   \\ fs []
-  \\ drule_all compile_semantics
-  \\ strip_tac \\ fs []
-  \\ drule compile_rel_semantics
-  \\ impl_keep_tac >-
-   (imp_res_tac pure_to_thunk_1ProofTheory.compile_rel_freevars
-    \\ fs [closed_def,pure_expTheory.closed_def])
-  \\ strip_tac \\ fs []
-  \\ drule case_force_semantics \\ fs []
-  \\ impl_keep_tac >-
-   (imp_res_tac thunk_case_liftProofTheory.compile_rel_freevars \\ fs [closed_def])
-  \\ strip_tac \\ fs []
-  \\ drule_at (Pos $ el 2) compile_case_proj_semantics
-  \\ impl_keep_tac
-  >- (drule exp_rel_NONE_freevars \\ fs [closed_def])
-  \\ strip_tac
-  \\ drule thunk_unthunkProofTheory.delay_force_semantics
-  \\ impl_keep_tac
-  >- (imp_res_tac compile_rel_closed \\ gvs [])
-  \\ strip_tac \\ fs []
-  \\ drule_all delay_force_closed \\ fs []
+  \\ imp_res_tac pure_to_thunk_1ProofTheory.compile_rel_freevars
+  \\ imp_res_tac thunk_unthunkProofTheory.delay_force_closed \\ gvs []
+  \\ imp_res_tac thunk_undelay_nextProofTheory.exp_rel_freevars
+  \\ imp_res_tac thunk_case_liftProofTheory.compile_rel_freevars
+  \\ imp_res_tac thunk_let_forceProofTheory.exp_rel_NONE_freevars
+  \\ imp_res_tac thunk_case_projProofTheory.compile_rel_closed \\ gvs []
+  \\ gvs [closed_def, pure_expTheory.closed_def]
+  \\ drule pure_to_thunk_1ProofTheory.compile_semantics \\ rw []
+  \\ drule thunk_unthunkProofTheory.delay_force_semantics_delayed \\ rw []
+  \\ drule thunk_undelay_nextProofTheory.undelay_semantics \\ rw []
+  \\ drule thunk_case_liftProofTheory.compile_rel_semantics \\ rw []
+  \\ drule thunk_let_forceProofTheory.case_force_semantics \\ rw []
+  \\ drule_at (Pat `proj_rel _ _`)
+       thunk_case_projProofTheory.compile_case_proj_semantics \\ rw []
+  \\ gvs [closed_def, pure_expTheory.closed_def]
 QED
 
 val _ = export_theory ();
